@prefix : <https://gotriple.eu/ontology/triple#> .
@prefix owl: <http://www.w3.org/2002/07/owl#> .
@prefix rdf: <http://www.w3.org/1999/02/22-rdf-syntax-ns#> .
@prefix xml: <http://www.w3.org/XML/1998/namespace> .
@prefix xsd: <http://www.w3.org/2001/XMLSchema#> .
@prefix rdfs: <http://www.w3.org/2000/01/rdf-schema#> .
@prefix triple: <https://gotriple.eu/ontology/triple#> .
@prefix cidoc: <http://www.cidoc-crm.org/cidoc-crm/> .
@prefix sshocro: <https://sshoc.eu/ontology/> .
@base <https://gotriple.eu/ontology/triple#> .

<https://gotriple.eu/ontology/triple> rdf:type owl:Ontology ;
                                       owl:versionIRI <https://gotriple.eu/ontology/triple/1.0.0> .

#################################################################
#    External Classes (CIDOC-CRM)
#################################################################


###  http://www.cidoc-crm.org/cidoc-crm/E31_Document
cidoc:E31_Document rdf:type owl:Class ;
                   rdfs:label "E31 Document"@en ;
                   rdfs:comment "CIDOC-CRM class representing identifiable immaterial items that make propositions about reality."@en .


###  http://www.cidoc-crm.org/cidoc-crm/E90_Symbolic_Object
cidoc:E90_Symbolic_Object rdf:type owl:Class ;
                          rdfs:label "E90 Symbolic Object"@en ;
                          rdfs:comment "CIDOC-CRM class representing symbols and any information object that can be identified."@en .


#################################################################
#    External Classes (SSHOCRo)
#################################################################

###  https://sshoc.eu/ontology/SHE3_SSH_Project
sshocro:SHE3_SSH_Project rdf:type owl:Class ;
                         rdfs:label "SHE3 SSH Project"@en ;
                         rdfs:comment "SSHOCRo class representing Social Sciences and Humanities research projects."@en .


###  https://sshoc.eu/ontology/SHE8_Publication
sshocro:SHE8_Publication rdf:type owl:Class ;
                         rdfs:label "SHE8 Publication"@en ;
                         rdfs:comment "SSHOCRo class representing scholarly publications in Social Sciences and Humanities."@en .


#################################################################
#    TRIPLE Class Alignments
#################################################################

###  https://gotriple.eu/ontology/triple#Document
triple:Document rdfs:subClassOf cidoc:E31_Document ,
                                sshocro:SHE8_Publication .


###  https://gotriple.eu/ontology/triple#Multimedia
triple:Multimedia rdfs:subClassOf cidoc:E90_Symbolic_Object .


###  https://gotriple.eu/ontology/triple#Software
triple:Software rdfs:subClassOf cidoc:E90_Symbolic_Object .


###  https://gotriple.eu/ontology/triple#SemanticArtefact
triple:SemanticArtefact rdfs:subClassOf cidoc:E90_Symbolic_Object .


###  https://gotriple.eu/ontology/triple#Project
triple:Project rdfs:subClassOf sshocro:SHE3_SSH_Project .
                               


###  Generated by the OWL API (version 4.5.25.2023-02-15T19:15:49Z) https://github.com/owlcs/owlapi
