@prefix : <https://gotriple.eu/ontology/triple#> .
@prefix owl: <http://www.w3.org/2002/07/owl#> .
@prefix rdf: <http://www.w3.org/1999/02/22-rdf-syntax-ns#> .
@prefix xsd: <http://www.w3.org/2001/XMLSchema#> .
@prefix rdfs: <http://www.w3.org/2000/01/rdf-schema#> .
@prefix triple: <https://gotriple.eu/ontology/triple#> .
@prefix foaf: <http://xmlns.com/foaf/0.1/> .
@prefix schema: <http://schema.org/> .
@prefix skos: <http://www.w3.org/2004/02/skos/core#> .
@prefix dc: <http://purl.org/dc/elements/1.1/> .
@base <https://gotriple.eu/ontology/triple#> .

<https://gotriple.eu/ontology/triple> rdf:type owl:Ontology ;
                                       owl:versionIRI <https://gotriple.eu/ontology/triple/1.0.0> .

#################################################################
#    Object Properties
#################################################################

###  http://purl.org/dc/elements/1.1/subject
dc:subject rdf:type owl:ObjectProperty ;
           rdfs:label "subject"@en ;
           rdfs:comment "The subject or topic of the document, using a term from a controlled vocabulary."@en .


###  http://purl.org/dc/elements/1.1/type
dc:type rdf:type owl:ObjectProperty ;
        rdfs:label "type"@en ;
        rdfs:comment "The type of the document (e.g., Article, Dataset, Book)."@en .


###  http://schema.org/conditionsOfAccess
schema:conditionsOfAccess rdf:type owl:ObjectProperty ;
                          rdfs:label "conditions of access"@en ;
                          rdfs:comment "The conditions under which the document can be accessed (e.g., Open Access, Restricted)."@en .


###  http://schema.org/license
schema:license rdf:type owl:ObjectProperty ;
               rdfs:label "license"@en ;
               rdfs:comment "The license under which the document is published (e.g., CC-BY, CC0)."@en .


###  http://www.w3.org/2004/02/skos/core#closeMatch
skos:closeMatch rdf:type owl:ObjectProperty ;
                rdfs:label "close match"@en ;
                rdfs:comment "A SKOS property indicating that two concepts are sufficiently similar to be used interchangeably in some contexts."@en .


###  http://www.w3.org/2004/02/skos/core#exactMatch
skos:exactMatch rdf:type owl:ObjectProperty ;
                rdfs:label "exact match"@en ;
                rdfs:comment "A SKOS property indicating that two concepts can be used interchangeably across all contexts."@en .


###  http://www.w3.org/2004/02/skos/core#inScheme
skos:inScheme rdf:type owl:ObjectProperty ;
              rdfs:label "in scheme"@en ;
              rdfs:comment "A SKOS property linking a concept to the concept scheme it belongs to."@en .


#################################################################
#    Annotation Properties
#################################################################

###  http://www.w3.org/2004/02/skos/core#definition
skos:definition rdf:type owl:AnnotationProperty ;
                rdfs:label "definition"@en ;
                rdfs:comment "A SKOS annotation property providing a complete explanation of the intended meaning of a concept."@en .


#################################################################
#    Classes
#################################################################

###  http://schema.org/CreativeWork
schema:CreativeWork rdf:type owl:Class ;
                    rdfs:label "Creative Work (Schema.org)"@en .


###  http://xmlns.com/foaf/0.1/Document
foaf:Document rdf:type owl:Class ;
              rdfs:label "Document (FOAF)"@en .


###  https://gotriple.eu/ontology/triple#Document
triple:Document rdf:type owl:Class ;
                rdfs:label "Document (Triple)"@en ;
                rdfs:comment "A document in the GoTriple platform, representing scholarly publications, research datasets, and other SSH research artifacts. It is a subclass of both schema:CreativeWork and foaf:Document."@en ;
                rdfs:subClassOf schema:CreativeWork ,
                                foaf:Document .


###  http://www.w3.org/2004/02/skos/core#Concept
skos:Concept rdf:type owl:Class ;
             rdfs:label "Concept (SKOS)"@en ;
             rdfs:comment "A SKOS concept representing a term in a controlled vocabulary."@en .


###  http://www.w3.org/2004/02/skos/core#ConceptScheme
skos:ConceptScheme rdf:type owl:Class ;
                   rdfs:label "Concept Scheme (SKOS)"@en ;
                   rdfs:comment "A SKOS concept scheme representing a controlled vocabulary (e.g., licenses, document types, disciplines)."@en .


###  Generated by the OWL API (version 4.5.26.2023-07-17T20:34:13Z) https://github.com/owlcs/owlapi
