@prefix datacite: <http://purl.org/spar/datacite/> .
@prefix dcat: <http://www.w3.org/ns/dcat#> .
@prefix dcterms: <http://purl.org/dc/terms/> .
@prefix foaf: <http://xmlns.com/foaf/0.1/> .
@prefix frapo: <http://purl.org/cerif/frapo/> .
@prefix litre: <http://purl.org/spar/literal/> .
@prefix mod: <https://w3id.org/mod#> .
@prefix oa: <http://www.w3.org/ns/oa#> .
@prefix owl: <http://www.w3.org/2002/07/owl#> .
@prefix rdf: <http://www.w3.org/1999/02/22-rdf-syntax-ns#> .
@prefix rdfs: <http://www.w3.org/2000/01/rdf-schema#> .
@prefix schema: <https://schema.org/> .
@prefix sioc: <http://rdfs.org/sioc/ns#> .
@prefix skos: <http://www.w3.org/2004/02/skos/core#> .
@prefix triple: <https://gotriple.eu/ontology/triple#> .
@prefix xsd: <http://www.w3.org/2001/XMLSchema#> .

schema:email a owl:DatatypeProperty ;
    rdfs:label "schema:email"@en ;
    rdfs:range xsd:string .

skos:closeMatch a owl:ObjectProperty ;
    rdfs:label "skos:closeMatch"@en ;
    rdfs:comment "A SKOS property indicating that two concepts are sufficiently similar to be used interchangeably in some contexts."@en .

skos:definition a owl:AnnotationProperty ;
    rdfs:label "skos:definition"@en ;
    rdfs:comment "A SKOS annotation property providing a complete explanation of the intended meaning of a concept."@en .

skos:exactMatch a owl:ObjectProperty ;
    rdfs:label "skos:exactMatch"@en ;
    rdfs:comment "A SKOS property indicating that two concepts can be used interchangeably across all contexts."@en .

skos:prefLabel a owl:AnnotationProperty .

oa:hasBody a owl:ObjectProperty ;
    rdfs:label "hasBody"@en .

oa:hasTarget a owl:ObjectProperty ;
    rdfs:label "hasTarget"@en .

oa:identifying a owl:NamedIndividual,
        oa:Motivation ;
    rdfs:label "identifying"@en .

oa:motivatedBy a owl:ObjectProperty ;
    rdfs:label "motivatedBy"@en .

<https://gotriple.eu/ontology/triple> a owl:Ontology ;
    rdfs:label "TRIPLE Ontology"@en ;
    dcterms:title "TRIPLE Ontology"@en ;
    dcterms:abstract "The TRIPLE Ontology defines a comprehensive model for representing Social Sciences and Humanities (SSH) resources in the GoTriple discovery platform, extending Schema.org and FOAF."@en ;
    dcterms:description "GoTriple is an advanced multilingual discovery platform specifically designed for the Social Sciences and Humanities (SSH) sector. The platform aggregates, processes, and semantically enriches diverse SSH resources including scholarly publications, research datasets, project descriptions, and researcher profiles from various European language repositories. The TRIPLE ontology serves as the data model for this platform, facilitating cross-disciplinary and cross-linguistic discovery and reuse of resources."@en ;
    dcterms:created "2021-12-01" ;
    dcterms:modified "2025-12-22" ;
    dcterms:creator "Alessandro Bertozzi" ;
    dcterms:contributor "Luca De Santis", "Silvio Peroni" ;
    owl:versionInfo "2.0.0" ;
    rdfs:comment "Comprehensive semantic representation of the GoTriple discovery platform's data model for Social Sciences and Humanities (SSH) research artifacts."@en ;
    owl:imports <https://gotriple.eu/ontology/triple/conditions_of_access#>,
        <https://gotriple.eu/ontology/triple/content_types#>,
        <https://gotriple.eu/ontology/triple/disciplines#>,
        <https://gotriple.eu/ontology/triple/licenses#>,
        <https://gotriple.eu/ontology/triple/project_types#> .

triple:Dataset a owl:Class ;
    rdfs:label "Dataset"@en,
        "Dataset (Triple)"@en ;
    rdfs:comment "A collection of data organized for research purposes in the Social Sciences and Humanities domain."@en,
        "A dataset in the GoTriple platform, representing research data with specific metadata including spatial coverage, temporal coverage, and distribution information. It is a subclass of dcat:Dataset."@en ;
    rdfs:subClassOf [ a owl:Restriction ;
            owl:allValuesFrom triple:Project ;
            owl:onProperty frapo:isOutputOf ],
        [ a owl:Restriction ;
            owl:allValuesFrom schema:CreativeWork ;
            owl:onProperty dcterms:isReferencedBy ],
        [ a owl:Restriction ;
            owl:allValuesFrom schema:Place ;
            owl:onProperty schema:spatialCoverage ],
        [ a owl:Restriction ;
            owl:allValuesFrom [ owl:unionOf ( foaf:Person foaf:Organization ) ] ;
            owl:onProperty schema:publisher ],
        [ a owl:Restriction ;
            owl:allValuesFrom [ owl:unionOf ( foaf:Person foaf:Organization ) ] ;
            owl:onProperty schema:provider ],
        [ a owl:Restriction ;
            owl:allValuesFrom owl:Thing ;
            owl:onProperty schema:funding ],
        [ a owl:Restriction ;
            owl:allValuesFrom schema:ContactPoint ;
            owl:onProperty schema:contactPoint ],
        [ a owl:Restriction ;
            owl:allValuesFrom owl:Thing ;
            owl:onProperty schema:mentions ],
        [ a owl:Restriction ;
            owl:allValuesFrom schema:DefinedTerm ;
            owl:onProperty schema:keywords ],
        [ a owl:Restriction ;
            owl:allValuesFrom owl:Thing ;
            owl:onProperty sioc:topic ],
        [ a owl:Restriction ;
            owl:allValuesFrom owl:Thing ;
            owl:onProperty dcterms:isReferencedBy ],
        [ a owl:Restriction ;
            owl:allValuesFrom xsd:string ;
            owl:onProperty schema:temporalCoverage ],
        [ a owl:Restriction ;
            owl:allValuesFrom xsd:string ;
            owl:onProperty schema:encodingFormat ],
        [ a owl:Restriction ;
            owl:allValuesFrom xsd:string ;
            owl:onProperty schema:size ],
        [ a owl:Restriction ;
            owl:allValuesFrom xsd:string ;
            owl:onProperty schema:creativeWorkStatus ],
        [ a owl:Restriction ;
            owl:allValuesFrom [ a owl:Class ;
                    owl:unionOf ( datacite:Identifier triple:ID triple:PID triple:OriginalIdentifier triple:DOI triple:Handle ) ] ;
            owl:onProperty datacite:hasIdentifier ],
        [ a owl:Restriction ;
            owl:allValuesFrom [ owl:unionOf ( foaf:Person foaf:Organization ) ] ;
            owl:onProperty schema:author ],
        [ a owl:Restriction ;
            owl:allValuesFrom rdf:langString ;
            owl:onProperty schema:headline ],
        [ a owl:Restriction ;
            owl:allValuesFrom rdf:langString ;
            owl:onProperty schema:abstract ],
        [ a owl:Restriction ;
            owl:allValuesFrom xsd:string ;
            owl:onProperty schema:knowsAbout ],
        [ a owl:Restriction ;
            owl:onProperty schema:inLanguage ;
            owl:someValuesFrom schema:Language ],
        [ a owl:Restriction ;
            owl:allValuesFrom xsd:date ;
            owl:onProperty schema:dateCreated ],
        [ a owl:Restriction ;
            owl:allValuesFrom xsd:date ;
            owl:onProperty schema:datePublished ],
        [ a owl:Restriction ;
            owl:allValuesFrom xsd:date ;
            owl:onProperty schema:dateModified ],
        [ a owl:Restriction ;
            owl:maxCardinality "1"^^xsd:nonNegativeInteger ;
            owl:onProperty schema:dateCreated ],
        [ a owl:Restriction ;
            owl:maxCardinality "1"^^xsd:nonNegativeInteger ;
            owl:onProperty schema:datePublished ],
        [ a owl:Restriction ;
            owl:maxCardinality "1"^^xsd:nonNegativeInteger ;
            owl:onProperty schema:dateModified ],
        [ a owl:Restriction ;
            owl:allValuesFrom xsd:string ;
            owl:onProperty schema:comment ],
        [ a owl:Restriction ;
            owl:allValuesFrom triple:Discipline ;
            owl:onProperty sioc:topic ],
        [ a owl:Restriction ;
            owl:allValuesFrom triple:Document ;
            owl:onProperty dcterms:isReferencedBy ],
        [ a owl:Restriction ;
            owl:allValuesFrom schema:URL ;
            owl:onProperty schema:mainEntityOfPage ],
        [ a owl:Restriction ;
            owl:allValuesFrom dcat:Distribution ;
            owl:onProperty dcat:distribution ],
        [ a owl:Restriction ;
            owl:allValuesFrom rdfs:Literal ;
            owl:onProperty dcat:bbox ],
        [ a owl:Restriction ;
            owl:allValuesFrom dcterms:ProvenanceStatement ;
            owl:onProperty dcterms:provenance ],
        [ a owl:Restriction ;
            owl:allValuesFrom triple:License ;
            owl:onProperty triple:hasLicense ],
        [ a owl:Restriction ;
            owl:allValuesFrom triple:AccessCondition ;
            owl:onProperty triple:hasAccessCondition ],
        [ a owl:Restriction ;
            owl:allValuesFrom triple:ContentType ;
            owl:onProperty triple:hasContentType ],
        [ a owl:Restriction ;
            owl:allValuesFrom [ owl:unionOf ( foaf:Person foaf:Organization ) ] ;
            owl:onProperty schema:contributor ],
        schema:Dataset,
        dcat:Dataset ;
    skos:exactMatch <http://purl.org/spar/fabio/Dataset>,
        <https://sshoc.eu/ontology/SHE1_Dataset> .

triple:MediaObject a owl:Class ;
    rdfs:label "Media Object"@en,
        "Media Object (Triple)"@en ;
    rdfs:comment "A media object such as an image, video, audio, or other multimedia content used in SSH research."@en,
        "A multimedia object in the GoTriple platform, representing various types of media files (audio, video, images) associated with scholarly works."@en ;
    rdfs:subClassOf [ a owl:Restriction ;
            owl:allValuesFrom triple:Project ;
            owl:onProperty frapo:isOutputOf ],
        [ a owl:Restriction ;
            owl:allValuesFrom schema:CreativeWork ;
            owl:onProperty dcterms:isReferencedBy ],
        [ a owl:Restriction ;
            owl:allValuesFrom [ owl:unionOf ( foaf:Person foaf:Organization ) ] ;
            owl:onProperty schema:publisher ],
        [ a owl:Restriction ;
            owl:allValuesFrom [ owl:unionOf ( foaf:Person foaf:Organization ) ] ;
            owl:onProperty schema:provider ],
        [ a owl:Restriction ;
            owl:allValuesFrom schema:DefinedTerm ;
            owl:onProperty schema:keywords ],
        [ a owl:Restriction ;
            owl:allValuesFrom schema:Place ;
            owl:onProperty schema:spatialCoverage ],
        [ a owl:Restriction ;
            owl:allValuesFrom rdf:langString ;
            owl:onProperty schema:headline ],
        [ a owl:Restriction ;
            owl:allValuesFrom rdf:langString ;
            owl:onProperty schema:abstract ],
        [ a owl:Restriction ;
            owl:allValuesFrom xsd:date ;
            owl:onProperty schema:dateCreated ],
        [ a owl:Restriction ;
            owl:allValuesFrom xsd:date ;
            owl:onProperty schema:datePublished ],
        [ a owl:Restriction ;
            owl:allValuesFrom xsd:date ;
            owl:onProperty schema:dateModified ],
        [ a owl:Restriction ;
            owl:maxCardinality "1"^^xsd:nonNegativeInteger ;
            owl:onProperty schema:dateCreated ],
        [ a owl:Restriction ;
            owl:maxCardinality "1"^^xsd:nonNegativeInteger ;
            owl:onProperty schema:datePublished ],
        [ a owl:Restriction ;
            owl:maxCardinality "1"^^xsd:nonNegativeInteger ;
            owl:onProperty schema:dateModified ],
        [ a owl:Restriction ;
            owl:allValuesFrom xsd:string ;
            owl:onProperty schema:encodingFormat ],
        [ a owl:Restriction ;
            owl:allValuesFrom xsd:string ;
            owl:onProperty schema:duration ],
        [ a owl:Restriction ;
            owl:allValuesFrom [ owl:unionOf ( foaf:Person foaf:Organization ) ] ;
            owl:onProperty schema:author ],
        [ a owl:Restriction ;
            owl:allValuesFrom xsd:string ;
            owl:onProperty schema:size ],
        [ a owl:Restriction ;
            owl:onProperty schema:inLanguage ;
            owl:someValuesFrom schema:Language ],
        [ a owl:Restriction ;
            owl:allValuesFrom triple:License ;
            owl:onProperty triple:hasLicense ],
        [ a owl:Restriction ;
            owl:allValuesFrom triple:AccessCondition ;
            owl:onProperty triple:hasAccessCondition ],
        [ a owl:Restriction ;
            owl:allValuesFrom xsd:string ;
            owl:onProperty schema:temporalCoverage ],
        [ a owl:Restriction ;
            owl:allValuesFrom xsd:string ;
            owl:onProperty schema:knowsAbout ],
        [ a owl:Restriction ;
            owl:allValuesFrom owl:Thing ;
            owl:onProperty schema:mentions ],
        [ a owl:Restriction ;
            owl:allValuesFrom [ a owl:Class ;
                    owl:unionOf ( datacite:Identifier triple:ID triple:PID triple:OriginalIdentifier triple:DOI triple:Handle ) ] ;
            owl:onProperty datacite:hasIdentifier ],
        [ a owl:Restriction ;
            owl:allValuesFrom triple:Discipline ;
            owl:onProperty sioc:topic ],
        [ a owl:Restriction ;
            owl:allValuesFrom triple:ContentType ;
            owl:onProperty triple:hasContentType ],
        [ a owl:Restriction ;
            owl:allValuesFrom triple:Document ;
            owl:onProperty dcterms:isReferencedBy ],
        [ a owl:Restriction ;
            owl:allValuesFrom schema:ContactPoint ;
            owl:onProperty schema:contactPoint ],
        [ a owl:Restriction ;
            owl:allValuesFrom [ owl:unionOf ( foaf:Person foaf:Organization ) ] ;
            owl:onProperty schema:contributor ],
        schema:MediaObject ;
    skos:closeMatch <http://purl.org/spar/fabio/Work>,
        <http://www.cidoc-crm.org/cidoc-crm/E90_Symbolic_Object> .

triple:Profile a owl:Class ;
    rdfs:label "profile"@en ;
    rdfs:comment "A profile representing either a person or an organization in the GoTriple system. Can be associated or not associated with a user account."@en ;
    rdfs:subClassOf [ a owl:Restriction ;
            owl:onClass datacite:Identifier ;
            owl:onProperty datacite:hasIdentifier ;
            owl:qualifiedCardinality "1"^^xsd:nonNegativeInteger ],
        [ a owl:Restriction ;
            owl:onDataRange xsd:string ;
            owl:onProperty schema:name ;
            owl:qualifiedCardinality "1"^^xsd:nonNegativeInteger ],
        [ a owl:Restriction ;
            owl:maxCardinality "1"^^xsd:nonNegativeInteger ;
            owl:onClass foaf:OnlineAccount ;
            owl:onProperty foaf:account ],
        [ owl:unionOf ( foaf:Person foaf:Organization ) ] ;
    skos:exactMatch foaf:Agent .

triple:SemanticArtefact a owl:Class ;
    rdfs:label "Semantic Artefact",
        "Semantic Artefact"@en ;
    rdfs:comment "A semantic artefact in the context of GoTriple platform, representing formal knowledge representations such as ontologies, controlled vocabularies, and other semantic resources used in SSH research"@en,
        "A semantic artefact in the context of GoTriple platform, representing formal knowledge representations such as ontologies, controlled vocabularies, and other semantic resources used in SSH research."@en ;
    rdfs:subClassOf [ a owl:Restriction ;
            owl:onProperty schema:headline ;
            owl:someValuesFrom rdf:langString ],
        [ a owl:Restriction ;
            owl:onProperty schema:abstract ;
            owl:someValuesFrom rdf:langString ],
        [ a owl:Restriction ;
            owl:allValuesFrom [ owl:unionOf ( foaf:Person foaf:Organization ) ] ;
            owl:onProperty schema:contributor ],
        [ a owl:Restriction ;
            owl:allValuesFrom [ owl:unionOf ( foaf:Person foaf:Organization ) ] ;
            owl:onProperty schema:author ],
        [ a owl:Restriction ;
            owl:onProperty schema:inLanguage ;
            owl:someValuesFrom schema:Language ],
        [ a owl:Restriction ;
            owl:allValuesFrom xsd:date ;
            owl:onProperty schema:dateCreated ],
        [ a owl:Restriction ;
            owl:allValuesFrom xsd:date ;
            owl:onProperty schema:datePublished ],
        [ a owl:Restriction ;
            owl:allValuesFrom xsd:date ;
            owl:onProperty schema:dateModified ],
        [ a owl:Restriction ;
            owl:maxCardinality "1"^^xsd:nonNegativeInteger ;
            owl:onProperty schema:dateCreated ],
        [ a owl:Restriction ;
            owl:maxCardinality "1"^^xsd:nonNegativeInteger ;
            owl:onProperty schema:datePublished ],
        [ a owl:Restriction ;
            owl:maxCardinality "1"^^xsd:nonNegativeInteger ;
            owl:onProperty schema:dateModified ],
        [ a owl:Restriction ;
            owl:maxCardinality "1"^^xsd:nonNegativeInteger ;
            owl:onProperty schema:version ],
        [ a owl:Restriction ;
            owl:allValuesFrom [ owl:unionOf ( foaf:Person foaf:Organization ) ] ;
            owl:onProperty schema:publisher ],
        [ a owl:Restriction ;
            owl:allValuesFrom [ owl:unionOf ( foaf:Person foaf:Organization ) ] ;
            owl:onProperty triple:aggregator ],
        [ a owl:Restriction ;
            owl:onProperty schema:fileFormat ;
            owl:someValuesFrom xsd:string ],
        [ a owl:Restriction ;
            owl:onProperty schema:encodingFormat ;
            owl:someValuesFrom xsd:string ],
        [ a owl:Restriction ;
            owl:allValuesFrom schema:ContactPoint ;
            owl:onProperty schema:contactPoint ],
        [ a owl:Restriction ;
            owl:maxCardinality "1"^^xsd:nonNegativeInteger ;
            owl:onProperty schema:creativeWorkStatus ],
        [ a owl:Restriction ;
            owl:allValuesFrom schema:DefinedTerm ;
            owl:onProperty schema:keywords ],
        [ a owl:Restriction ;
            owl:allValuesFrom triple:Document ;
            owl:onProperty dcterms:isReferencedBy ],
        [ a owl:Restriction ;
            owl:allValuesFrom [ a owl:Class ;
                    owl:unionOf ( datacite:Identifier triple:ID triple:PID triple:OriginalIdentifier triple:DOI triple:Handle triple:URI ) ] ;
            owl:onProperty datacite:hasIdentifier ],
        [ a owl:Restriction ;
            owl:allValuesFrom schema:Place ;
            owl:onProperty schema:spatialCoverage ],
        [ a owl:Restriction ;
            owl:allValuesFrom triple:Discipline ;
            owl:onProperty sioc:topic ],
        [ a owl:Restriction ;
            owl:allValuesFrom triple:License ;
            owl:onProperty triple:hasLicense ],
        [ a owl:Restriction ;
            owl:allValuesFrom triple:AccessCondition ;
            owl:onProperty triple:hasAccessCondition ],
        [ a owl:Restriction ;
            owl:allValuesFrom triple:ContentType ;
            owl:onProperty triple:hasContentType ],
        [ a owl:Restriction ;
            owl:allValuesFrom triple:Project ;
            owl:onProperty frapo:isOutputOf ],
        [ a owl:Restriction ;
            owl:allValuesFrom schema:CreativeWork ;
            owl:onProperty dcterms:isReferencedBy ],
        schema:CreativeWork,
        mod:SemanticArtefact ;
    skos:closeMatch <http://purl.org/spar/fabio/Work>,
        <http://www.cidoc-crm.org/cidoc-crm/E90_Symbolic_Object> .

triple:full_text_url_schema a datacite:IdentifierScheme,
        owl:NamedIndividual ;
    rdfs:label "Full Text URL"@en ;
    rdfs:comment "URL providing direct access to the full content of the document."@en .

triple:isDiscarded a owl:DatatypeProperty ;
    rdfs:label "is discarded"@en ;
    rdfs:comment "A boolean flag indicating whether an entity (author or keyword) has been marked as discarded and should not be used for search/filtering."@en ;
    rdfs:range xsd:boolean .

triple:landing_page_url_schema a datacite:IdentifierScheme,
        owl:NamedIndividual ;
    rdfs:label "Landing Page URL"@en ;
    rdfs:comment "URL of the landing page containing metadata and descriptive information about the document."@en .

triple:source_url_schema a datacite:IdentifierScheme,
        owl:NamedIndividual ;
    rdfs:label "Source URL"@en ;
    rdfs:comment "URL of the original publication location or source repository."@en .

frapo:Grant a owl:Class ;
    rdfs:label "frapo:Grant"@en ;
    rdfs:comment "A funding grant."@en .

dcterms:provenance a owl:ObjectProperty ;
    rdfs:label "dcterms:provenance"@en ;
    rdfs:comment "A statement of any changes in ownership and custody of the resource since its creation that are significant for its authenticity, integrity, and interpretation."@en ;
    rdfs:range dcterms:ProvenanceStatement .

dcterms:source a owl:ObjectProperty .

datacite:doi a datacite:IdentifierScheme,
        owl:NamedIndividual ;
    rdfs:label "datacite:doi"@en ;
    rdfs:comment "Digital Object Identifier - a persistent identifier for digital objects maintained by the International DOI Foundation."@en .

datacite:handle a datacite:IdentifierScheme,
        owl:NamedIndividual ;
    rdfs:label "datacite:handle"@en ;
    rdfs:comment "Handle System - a persistent identifier infrastructure for managing digital objects."@en .

datacite:isbn a datacite:IdentifierScheme,
        owl:NamedIndividual ;
    rdfs:label "datacite:isbn"@en ;
    rdfs:comment "International Standard Book Number - a numeric identifier for books and book-like products."@en .

datacite:issn a datacite:IdentifierScheme,
        owl:NamedIndividual ;
    rdfs:label "datacite:issn"@en ;
    rdfs:comment "International Standard Serial Number - an eight-digit identifier for serial publications."@en .

datacite:uri a datacite:IdentifierScheme,
        owl:NamedIndividual ;
    rdfs:label "datacite:uri"@en ;
    rdfs:comment "Uniform Resource Identifier - a string of characters that unambiguously identifies a particular resource."@en .

<http://purl.org/spar/fabio/Dataset> a owl:Class ;
    rdfs:label "fabio:Dataset"@en ;
    rdfs:comment "A dataset."@en .

<http://purl.org/spar/fabio/ScholarlyWork> a owl:Class ;
    rdfs:label "fabio:ScholarlyWork"@en ;
    rdfs:comment "A scholarly work."@en .

schema:Grant a owl:Class ;
    rdfs:label "schema:Grant"@en ;
    rdfs:comment "A grant, typically financial or otherwise quantifiable, of resources"@en ;
    rdfs:subClassOf [ a owl:Restriction ;
            owl:allValuesFrom [ owl:unionOf ( foaf:Person foaf:Organization ) ] ;
            owl:onProperty schema:funder ],
        [ a owl:Restriction ;
            owl:allValuesFrom [ owl:unionOf ( foaf:Person foaf:Organization ) ] ;
            owl:onProperty schema:sponsor ] .

schema:MediaObject a owl:Class ;
    rdfs:label "schema:MediaObject"@en ;
    rdfs:comment "A media object, such as an image, video, or audio object embedded in a web page or a downloadable dataset. Note that a creative work may have many media objects associated with it on the same web page."@en .

schema:Person a owl:Class ;
    rdfs:label "Person"@en,
        "schema:Person"@en .

schema:Project a owl:Class ;
    rdfs:label "schema:Project"@en ;
    rdfs:comment "An enterprise (potentially individual but typically collaborative), planned to achieve a particular aim."@en .

schema:Text a rdfs:Datatype .

schema:about a owl:ObjectProperty ;
    rdfs:label "schema:about"@en ;
    rdfs:comment "The subject matter of the content"@en .

schema:alternateName a owl:DatatypeProperty ;
    rdfs:label "schema:alternateName"@en ;
    rdfs:comment "An alias for the item"@en ;
    rdfs:range rdf:langString .

schema:comment a owl:DatatypeProperty ;
    rdfs:label "schema:comment"@en ;
    rdfs:comment "Comments, typically from users."@en .

schema:description a owl:DatatypeProperty ;
    rdfs:label "schema:description"@en ;
    rdfs:comment "A description of the item"@en ;
    rdfs:range rdf:langString .

schema:duration a owl:DatatypeProperty ;
    rdfs:label "schema:duration"@en ;
    rdfs:comment "The duration of the item (movie, audio recording, event, etc.) in ISO 8601 duration format."@en .

schema:fileFormat a owl:DatatypeProperty ;
    rdfs:label "schema:fileFormat" ;
    rdfs:comment "Media type, typically MIME format"@en ;
    rdfs:range xsd:string .

schema:organizer a owl:ObjectProperty ;
    rdfs:label "schema:organizer"@en ;
    rdfs:comment "The organization who organizes the event or project."@en ;
    rdfs:range schema:Organization .

schema:sponsor a owl:ObjectProperty ;
    rdfs:label "schema:sponsor"@en ;
    rdfs:comment "A person or organization that supports a thing through a pledge, promise, or financial contribution"@en .

schema:version a owl:DatatypeProperty ;
    rdfs:label "schema:version" ;
    rdfs:comment "The version of the CreativeWork"@en ;
    rdfs:range xsd:string .

<http://www.cidoc-crm.org/cidoc-crm/E31_Document> a owl:Class ;
    rdfs:label "E31 Document"@en .

<http://www.cidoc-crm.org/cidoc-crm/E7_Activity> a owl:Class ;
    rdfs:label "E7 Activity"@en .

dcat:bbox a owl:DatatypeProperty ;
    rdfs:label "dcat:bbox"@en ;
    rdfs:comment "The bounding box of the dataset, expressed as a literal (e.g., WKT)."@en ;
    rdfs:range rdfs:Literal .

oa:Annotation a owl:Class ;
    rdfs:label "Annotation"@en .

oa:Motivation a owl:Class ;
    rdfs:label "Motivation"@en .

foaf:Agent a owl:Class ;
    rdfs:label "foaf:Agent"@en ;
    rdfs:comment "An agent (person or organization)."@en .

foaf:Document a owl:Class ;
    rdfs:label "foaf:Document"@en .

foaf:OnlineAccount a owl:Class ;
    rdfs:label "foaf:OnlineAccount"@en ;
    rdfs:subClassOf [ a owl:Restriction ;
            owl:onClass datacite:Identifier ;
            owl:onProperty datacite:hasIdentifier ;
            owl:qualifiedCardinality "1"^^xsd:nonNegativeInteger ] .

foaf:account a owl:ObjectProperty ;
    rdfs:label "foaf:account"@en ;
    rdfs:comment "Indicates an account held by this agent"@en .

triple:ISBN a owl:Class ;
    rdfs:label "ISBN"@en ;
    rdfs:comment "International Standard Book Number - a numeric commercial book identifier assigned to books and book-like products."@en ;
    rdfs:subClassOf [ a owl:Restriction ;
            owl:onDataRange xsd:string ;
            owl:onProperty litre:hasLiteralValue ;
            owl:qualifiedCardinality "1"^^xsd:nonNegativeInteger ],
        [ a owl:Restriction ;
            owl:hasValue datacite:isbn ;
            owl:onProperty datacite:usesIdentifierScheme ],
        datacite:Identifier .

triple:ISSN a owl:Class ;
    rdfs:label "ISSN"@en ;
    rdfs:comment "International Standard Serial Number - an eight-digit identifier used to uniquely identify serial publications."@en ;
    rdfs:subClassOf [ a owl:Restriction ;
            owl:onDataRange xsd:string ;
            owl:onProperty litre:hasLiteralValue ;
            owl:qualifiedCardinality "1"^^xsd:nonNegativeInteger ],
        [ a owl:Restriction ;
            owl:hasValue datacite:issn ;
            owl:onProperty datacite:usesIdentifierScheme ],
        datacite:Identifier .

triple:URI a owl:Class ;
    rdfs:label "URI"@en ;
    rdfs:comment "Uniform Resource Identifier - a string of characters that unambiguously identifies a particular resource."@en ;
    rdfs:subClassOf [ a owl:Restriction ;
            owl:onDataRange xsd:string ;
            owl:onProperty litre:hasLiteralValue ;
            owl:qualifiedCardinality "1"^^xsd:nonNegativeInteger ],
        [ a owl:Restriction ;
            owl:hasValue datacite:uri ;
            owl:onProperty datacite:usesIdentifierScheme ],
        datacite:Identifier .

triple:hasProjectType a owl:ObjectProperty ;
    rdfs:label "has project type"@en ;
    rdfs:range triple:ProjectType ;
    rdfs:subPropertyOf dcterms:type .

triple:inCluster a owl:ObjectProperty ;
    rdfs:label "in cluster"@en ;
    rdfs:comment "Associates a document with its cluster (for deduplication purposes)."@en ;
    rdfs:domain triple:Document ;
    rdfs:range triple:Cluster .

<https://sshoc.eu/ontology/SHE1_Dataset> a owl:Class ;
    rdfs:label "SHE1 Dataset"@en .

<https://sshoc.eu/ontology/SHE3_SSH_Project> a owl:Class ;
    rdfs:label "SHE3 SSH Project"@en .

<https://sshoc.eu/ontology/SHE8_Publication> a owl:Class ;
    rdfs:label "SHE8 Publication"@en .

dcterms:ProvenanceStatement a owl:Class ;
    rdfs:label "dcterms:ProvenanceStatement"@en ;
    rdfs:comment "A statement of any changes in ownership and custody of the resource since its creation that are significant for its authenticity, integrity, and interpretation."@en .

<http://purl.org/spar/fabio/Work> a owl:Class ;
    rdfs:label "fabio:Work"@en ;
    rdfs:comment "A work."@en .

schema:Organization a owl:Class ;
    rdfs:label "schema:Organization"@en .

schema:Thing a owl:Class ;
    rdfs:label "schema:Thing"@en .

schema:creativeWorkStatus a owl:DatatypeProperty ;
    rdfs:label "schema:creativeWorkStatus",
        "schema:creativeWorkStatus"@en ;
    rdfs:comment "The status of a creative work in terms of its stage in a lifecycle"@en,
        "The status of a creative work in terms of its stage in a lifecycle."@en ;
    rdfs:range xsd:string .

schema:endDate a owl:DatatypeProperty ;
    rdfs:label "schema:endDate"@en ;
    rdfs:comment "The end date and time of the item"@en ;
    rdfs:range xsd:date .

schema:funder a owl:ObjectProperty ;
    rdfs:label "schema:funder"@en ;
    rdfs:comment "A person or organization that supports something through some kind of financial contribution"@en,
        "A person or organization that supports through funding"@en ;
    rdfs:range [ owl:unionOf ( foaf:Person foaf:Organization ) ] .

schema:funding a owl:ObjectProperty ;
    rdfs:label "schema:funding"@en ;
    rdfs:comment "A Grant that directly or indirectly provide funding or sponsorship for this item."@en,
        "A grant, typically financial or otherwise quantifiable, of resources"@en .

schema:mainEntityOfPage a owl:DatatypeProperty ;
    rdfs:label "schema:mainEntityOfPage"@en ;
    rdfs:comment "Indicates a page (or other CreativeWork) for which this thing is the main entity being described."@en ;
    rdfs:range schema:URL .

schema:size a owl:DatatypeProperty ;
    rdfs:label "schema:size"@en ;
    rdfs:comment "A standardized size of a product or creative work, specified either through a simple textual string or a QuantitativeValue."@en,
        "A standardized size of a product or creative work."@en .

schema:startDate a owl:DatatypeProperty ;
    rdfs:label "schema:startDate"@en ;
    rdfs:comment "The start date and time of the item"@en ;
    rdfs:range xsd:date .

<http://www.cidoc-crm.org/cidoc-crm/E90_Symbolic_Object> a owl:Class ;
    rdfs:label "E90 Symbolic Object"@en .

triple:Cluster a owl:Class ;
    rdfs:label "Cluster"@en ;
    rdfs:comment "A cluster groups multiple documents from different sources that represent the same scholarly work. Used for deduplication."@en ;
    rdfs:subClassOf [ a owl:Restriction ;
            owl:onClass datacite:Identifier ;
            owl:onProperty datacite:hasIdentifier ;
            owl:qualifiedCardinality "1"^^xsd:nonNegativeInteger ] .

triple:ProjectType a owl:Class ;
    rdfs:label "Project Type"@en ;
    rdfs:subClassOf skos:Concept .

triple:aggregator a owl:ObjectProperty ;
    rdfs:label "aggregator"@en ;
    rdfs:comment "An aggregator that collates resources from different sources"@en ;
    rdfs:range [ owl:unionOf ( foaf:Person foaf:Organization ) ] ;
    rdfs:subPropertyOf schema:contributor .

datacite:local-resource-identifier-scheme a datacite:IdentifierScheme,
        owl:NamedIndividual ;
    rdfs:label "datacite:local-resource-identifier-scheme"@en ;
    rdfs:comment "Local resource identifier scheme for platform-specific identifiers as defined by DataCite."@en .

schema:URL a rdfs:Datatype ;
    rdfs:label "schema:URL"@en ;
    rdfs:comment "Data type: URL."@en .

schema:knowsAbout a owl:DatatypeProperty,
        owl:ObjectProperty ;
    rdfs:label "schema:knowsAbout"@en ;
    rdfs:comment "Of a Person, and less typically of an Organization, to indicate a topic that is known about - suggested for areas of expertise."@en,
        "Of a Person, and less typically of an Organization, to indicate a topic that is known about."@en ;
    rdfs:range xsd:string,
        skos:Concept .

schema:mentions a owl:ObjectProperty ;
    rdfs:label "mentions"@en,
        "schema:mentions"@en ;
    rdfs:comment "Indicates that the CreativeWork contains a reference to, but is not necessarily about a particular thing."@en ;
    rdfs:range owl:Thing .

schema:provider a owl:ObjectProperty ;
    rdfs:label "schema:provider"@en ;
    rdfs:comment "The service provider, organization, or individual that provides the data"@en,
        "The service provider, service operator, or service performer."@en,
        "The service provider, service operator, or service performer; the goods producer."@en ;
    rdfs:range [ owl:unionOf ( foaf:Person foaf:Organization ) ] .

schema:temporalCoverage a owl:DatatypeProperty ;
    rdfs:label "schema:temporalCoverage",
        "schema:temporalCoverage"@en ;
    rdfs:comment "The temporalCoverage of a CreativeWork indicates the period that the content applies to."@en ;
    rdfs:range xsd:string .

frapo:isOutputOf a owl:ObjectProperty ;
    rdfs:label "frapo:isOutputOf"@en ;
    rdfs:comment "Indicates that a research output is the result of a particular project."@en ;
    rdfs:range triple:Project .

schema:abstract a owl:DatatypeProperty ;
    rdfs:label "schema:abstract",
        "schema:abstract"@en ;
    rdfs:comment "An abstract is a short description that summarizes a CreativeWork"@en,
        "An abstract is a short description that summarizes a CreativeWork."@en ;
    rdfs:range rdf:langString .

schema:author a owl:ObjectProperty ;
    rdfs:label "schema:author"@en ;
    rdfs:comment "The author of this content"@en,
        "The author of this content or rating."@en,
        "The author of this content."@en ;
    rdfs:range [ owl:unionOf ( foaf:Person foaf:Organization ) ],
        [ owl:unionOf ( foaf:Person foaf:Organization ) ] ;
    rdfs:subPropertyOf schema:creator .

schema:encodingFormat a owl:DatatypeProperty ;
    rdfs:label "schema:encodingFormat",
        "schema:encodingFormat"@en ;
    rdfs:comment "Media type typically expressed using a MIME format"@en,
        "Media type typically expressed using a MIME format."@en ;
    rdfs:range xsd:string .

schema:headline a owl:DatatypeProperty ;
    rdfs:label "schema:headline",
        "schema:headline"@en ;
    rdfs:comment "Headline of the article"@en,
        "Headline of the article."@en ;
    rdfs:range rdf:langString .

schema:publisher a owl:ObjectProperty ;
    rdfs:label "schema:publisher"@en ;
    rdfs:comment "The publisher of the creative work"@en,
        "The publisher of the creative work."@en ;
    rdfs:range [ owl:unionOf ( foaf:Person foaf:Organization ) ],
        [ owl:unionOf ( foaf:Person foaf:Organization ) ] .

schema:spatialCoverage a owl:ObjectProperty ;
    rdfs:label "schema:spatialCoverage",
        "schema:spatialCoverage"@en ;
    rdfs:comment "The spatialCoverage of a CreativeWork indicates the place(s) which are the focus of the content."@en ;
    rdfs:range schema:Place .

triple:DOI a owl:Class ;
    rdfs:label "DOI"@en ;
    rdfs:comment "Digital Object Identifier - a persistent identifier for digital objects maintained by the International DOI Foundation."@en ;
    rdfs:subClassOf [ a owl:Restriction ;
            owl:onDataRange xsd:string ;
            owl:onProperty litre:hasLiteralValue ;
            owl:qualifiedCardinality "1"^^xsd:nonNegativeInteger ],
        [ a owl:Restriction ;
            owl:hasValue datacite:doi ;
            owl:onProperty datacite:usesIdentifierScheme ],
        datacite:Identifier .

triple:Discipline a owl:Class ;
    rdfs:label "Discipline"@en ;
    rdfs:subClassOf skos:Concept .

triple:Document a owl:Class ;
    rdfs:label "Document"@en,
        "Document (Triple)"@en ;
    rdfs:comment "A document in the GoTriple platform, representing scholarly publications and research outputs."@en,
        "A document in the GoTriple platform, representing scholarly publications, research datasets, and other SSH research artifacts."@en,
        "A document in the GoTriple platform, representing scholarly publications, research datasets, and other SSH research artifacts. It is a subclass of both schema:CreativeWork and foaf:Document."@en ;
    rdfs:subClassOf [ a owl:Restriction ;
            owl:allValuesFrom [ owl:unionOf ( foaf:Person foaf:Organization ) ] ;
            owl:onProperty schema:author ],
        [ a owl:Restriction ;
            owl:allValuesFrom [ owl:unionOf ( foaf:Person foaf:Organization ) ] ;
            owl:onProperty schema:contributor ],
        [ a owl:Restriction ;
            owl:allValuesFrom [ owl:unionOf ( foaf:Person foaf:Organization ) ] ;
            owl:onProperty schema:publisher ],
        [ a owl:Restriction ;
            owl:allValuesFrom [ owl:unionOf ( foaf:Person foaf:Organization ) ] ;
            owl:onProperty schema:funder ],
        [ a owl:Restriction ;
            owl:allValuesFrom [ owl:unionOf ( foaf:Person foaf:Organization ) ] ;
            owl:onProperty schema:provider ],
        [ a owl:Restriction ;
            owl:allValuesFrom [ owl:unionOf ( foaf:Person foaf:Organization ) ] ;
            owl:onProperty triple:aggregator ],
        [ a owl:Restriction ;
            owl:allValuesFrom schema:ContactPoint ;
            owl:onProperty schema:contactPoint ],
        [ a owl:Restriction ;
            owl:allValuesFrom triple:Project ;
            owl:onProperty frapo:isOutputOf ],
        [ a owl:Restriction ;
            owl:allValuesFrom triple:Discipline ;
            owl:onProperty sioc:topic ],
        [ a owl:Restriction ;
            owl:allValuesFrom triple:License ;
            owl:onProperty triple:hasLicense ],
        [ a owl:Restriction ;
            owl:allValuesFrom triple:AccessCondition ;
            owl:onProperty triple:hasAccessCondition ],
        [ a owl:Restriction ;
            owl:allValuesFrom triple:ContentType ;
            owl:onProperty triple:hasContentType ],
        [ a owl:Restriction ;
            owl:allValuesFrom [ a owl:Class ;
                    owl:unionOf ( datacite:Identifier triple:DOI triple:Handle triple:ISSN triple:ISBN ) ] ;
            owl:onProperty datacite:hasIdentifier ],
        [ a owl:Restriction ;
            owl:onProperty datacite:hasIdentifier ;
            owl:someValuesFrom triple:OriginalIdentifier ],
        [ a owl:Restriction ;
            owl:onProperty schema:inLanguage ;
            owl:someValuesFrom schema:Language ],
        [ a owl:Restriction ;
            owl:onProperty schema:headline ;
            owl:someValuesFrom rdf:langString ],
        [ a owl:Restriction ;
            owl:onProperty schema:abstract ;
            owl:someValuesFrom rdf:langString ],
        [ a owl:Restriction ;
            owl:onProperty schema:encodingFormat ;
            owl:someValuesFrom xsd:string ],
        [ a owl:Restriction ;
            owl:onProperty sioc:topic ;
            owl:someValuesFrom skos:Concept ],
        [ a owl:Restriction ;
            owl:onProperty dcterms:source ;
            owl:someValuesFrom owl:Thing ],
        [ a owl:Restriction ;
            owl:onProperty datacite:hasIdentifier ;
            owl:someValuesFrom triple:ID ],
        [ a owl:Restriction ;
            owl:onProperty datacite:hasIdentifier ;
            owl:someValuesFrom triple:PID ],
        [ a owl:Restriction ;
            owl:onClass triple:Cluster ;
            owl:onProperty triple:inCluster ;
            owl:qualifiedCardinality "1"^^xsd:nonNegativeInteger ],
        [ a owl:Restriction ;
            owl:onProperty schema:keywords ;
            owl:someValuesFrom schema:DefinedTerm ],
        [ a owl:Restriction ;
            owl:onProperty schema:spatialCoverage ;
            owl:someValuesFrom schema:Place ],
        [ a owl:Restriction ;
            owl:onProperty schema:temporalCoverage ;
            owl:someValuesFrom xsd:string ],
        [ a owl:Restriction ;
            owl:onProperty schema:mentions ;
            owl:someValuesFrom oa:Annotation ],
        schema:CreativeWork,
        foaf:Document ;
    skos:exactMatch <http://purl.org/spar/fabio/ScholarlyWork>,
        <http://www.cidoc-crm.org/cidoc-crm/E31_Document>,
        <https://sshoc.eu/ontology/SHE8_Publication> .

triple:Handle a owl:Class ;
    rdfs:label "Handle"@en ;
    rdfs:comment "Handle System - a persistent identifier infrastructure for managing digital objects."@en ;
    rdfs:subClassOf [ a owl:Restriction ;
            owl:onDataRange xsd:string ;
            owl:onProperty litre:hasLiteralValue ;
            owl:qualifiedCardinality "1"^^xsd:nonNegativeInteger ],
        [ a owl:Restriction ;
            owl:hasValue datacite:handle ;
            owl:onProperty datacite:usesIdentifierScheme ],
        datacite:Identifier .

triple:hasAccessCondition a owl:ObjectProperty ;
    rdfs:label "has access condition"@en ;
    rdfs:range triple:AccessCondition ;
    rdfs:subPropertyOf dcterms:accessRights .

triple:hasContentType a owl:ObjectProperty ;
    rdfs:label "has content type"@en ;
    rdfs:range triple:ContentType ;
    rdfs:subPropertyOf dcterms:type .

triple:hasLicense a owl:ObjectProperty ;
    rdfs:label "has license"@en ;
    rdfs:range triple:License ;
    rdfs:subPropertyOf dcterms:license .

schema:CreativeWork a owl:Class ;
    rdfs:label "schema:CreativeWork"@en .

schema:Place a owl:Class ;
    rdfs:label "Place"@en,
        "schema:Place"@en ;
    rdfs:comment "Entities that have a somewhat fixed, physical extension."@en ;
    rdfs:subClassOf [ a owl:Restriction ;
            owl:onProperty schema:name ;
            owl:someValuesFrom xsd:string ] .

schema:contactPoint a owl:ObjectProperty ;
    rdfs:label "schema:contactPoint"@en ;
    rdfs:comment "A contact point for a person or organization."@en ;
    rdfs:range schema:ContactPoint .

schema:contributor a owl:ObjectProperty ;
    rdfs:label "schema:contributor"@en ;
    rdfs:comment "A secondary contributor to the CreativeWork"@en,
        "A secondary contributor to the CreativeWork or Event."@en,
        "A secondary contributor to the CreativeWork."@en,
        "A secondary contributor to the creative work or event."@en ;
    rdfs:range [ owl:unionOf ( foaf:Person foaf:Organization ) ],
        [ owl:unionOf ( foaf:Person foaf:Organization ) ] .

schema:inLanguage a owl:ObjectProperty ;
    rdfs:label "schema:inLanguage"@en ;
    rdfs:comment "The language of the content or performance or used in an action."@en ;
    rdfs:range schema:Language .

schema:keywords a owl:ObjectProperty ;
    rdfs:label "schema:keywords",
        "schema:keywords"@en ;
    rdfs:comment "Keywords or tags used to describe content"@en,
        "Keywords or tags used to describe this content"@en,
        "Keywords or tags used to describe this content."@en ;
    rdfs:range schema:DefinedTerm .

triple:AccessCondition a owl:Class ;
    rdfs:label "Access Condition"@en ;
    rdfs:subClassOf dcterms:RightsStatement,
        skos:Concept .

triple:ContentType a owl:Class ;
    rdfs:label "Content Type"@en ;
    rdfs:subClassOf skos:Concept .

triple:ID a owl:Class ;
    rdfs:label "ID"@en,
        "Internal ID"@en ;
    rdfs:comment "Internal identifier used within the GoTriple platform for resource management."@en ;
    rdfs:subClassOf [ a owl:Restriction ;
            owl:onDataRange xsd:string ;
            owl:onProperty litre:hasLiteralValue ;
            owl:qualifiedCardinality "1"^^xsd:nonNegativeInteger ],
        [ a owl:Restriction ;
            owl:hasValue datacite:local-resource-identifier-scheme ;
            owl:onProperty datacite:usesIdentifierScheme ],
        datacite:Identifier .

triple:License a owl:Class ;
    rdfs:label "License"@en ;
    rdfs:subClassOf dcterms:LicenseDocument,
        skos:Concept .

triple:OriginalIdentifier a owl:Class ;
    rdfs:label "Original Identifier"@en,
        "OriginalIdentifier"@en ;
    rdfs:comment "Original identifier from the source system where the resource was harvested."@en ;
    rdfs:subClassOf [ a owl:Restriction ;
            owl:onDataRange xsd:string ;
            owl:onProperty litre:hasLiteralValue ;
            owl:qualifiedCardinality "1"^^xsd:nonNegativeInteger ],
        [ a owl:Restriction ;
            owl:hasValue datacite:local-resource-identifier-scheme ;
            owl:onProperty datacite:usesIdentifierScheme ],
        datacite:Identifier .

triple:PID a owl:Class ;
    rdfs:label "PID"@en,
        "Persistent ID"@en ;
    rdfs:comment "Persistent identifier generated and exposed externally by the GoTriple platform."@en ;
    rdfs:subClassOf [ a owl:Restriction ;
            owl:onDataRange xsd:string ;
            owl:onProperty litre:hasLiteralValue ;
            owl:qualifiedCardinality "1"^^xsd:nonNegativeInteger ],
        [ a owl:Restriction ;
            owl:hasValue datacite:local-resource-identifier-scheme ;
            owl:onProperty datacite:usesIdentifierScheme ],
        datacite:Identifier .

triple:Project a owl:Class ;
    rdfs:label "Project"@en,
        "Project (Triple)"@en ;
    rdfs:comment "A research project in the Social Sciences and Humanities domain integrated into the GoTriple platform."@en,
        "A research project in the Social Sciences and Humanities domain integrated into the GoTriple platform. It is a subclass of schema:Project."@en ;
    rdfs:subClassOf [ a owl:Restriction ;
            owl:allValuesFrom [ a owl:Class ;
                    owl:unionOf ( datacite:Identifier triple:ID triple:PID triple:OriginalIdentifier ) ] ;
            owl:onProperty datacite:hasIdentifier ],
        [ a owl:Restriction ;
            owl:maxCardinality "1"^^xsd:nonNegativeInteger ;
            owl:onProperty schema:startDate ],
        [ a owl:Restriction ;
            owl:allValuesFrom xsd:date ;
            owl:onProperty schema:startDate ],
        [ a owl:Restriction ;
            owl:allValuesFrom xsd:date ;
            owl:onProperty schema:endDate ],
        [ a owl:Restriction ;
            owl:maxCardinality "1"^^xsd:nonNegativeInteger ;
            owl:onProperty schema:endDate ],
        [ a owl:Restriction ;
            owl:allValuesFrom schema:Grant ;
            owl:onProperty schema:funding ],
        [ a owl:Restriction ;
            owl:allValuesFrom skos:Concept ;
            owl:onProperty schema:about ],
        [ a owl:Restriction ;
            owl:allValuesFrom schema:DefinedTerm ;
            owl:onProperty schema:keywords ],
        [ a owl:Restriction ;
            owl:allValuesFrom rdf:langString ;
            owl:onProperty schema:description ],
        [ a owl:Restriction ;
            owl:allValuesFrom rdf:langString ;
            owl:onProperty schema:alternateName ],
        [ a owl:Restriction ;
            owl:allValuesFrom schema:Organization ;
            owl:onProperty schema:organizer ],
        [ a owl:Restriction ;
            owl:allValuesFrom skos:Concept ;
            owl:onProperty schema:knowsAbout ],
        [ a owl:Restriction ;
            owl:allValuesFrom schema:URL ;
            owl:onProperty schema:mainEntityOfPage ],
        [ a owl:Restriction ;
            owl:onProperty schema:inLanguage ;
            owl:someValuesFrom schema:Language ],
        [ a owl:Restriction ;
            owl:maxCardinality "1"^^xsd:nonNegativeInteger ;
            owl:onProperty schema:dateCreated ],
        [ a owl:Restriction ;
            owl:allValuesFrom xsd:date ;
            owl:onProperty schema:dateCreated ],
        [ a owl:Restriction ;
            owl:maxCardinality "1"^^xsd:nonNegativeInteger ;
            owl:onProperty schema:dateModified ],
        [ a owl:Restriction ;
            owl:allValuesFrom xsd:date ;
            owl:onProperty schema:dateModified ],
        [ a owl:Restriction ;
            owl:allValuesFrom schema:ContactPoint ;
            owl:onProperty schema:contactPoint ],
        [ a owl:Restriction ;
            owl:allValuesFrom triple:ProjectType ;
            owl:onProperty triple:hasProjectType ],
        [ a owl:Restriction ;
            owl:minCardinality "1"^^xsd:nonNegativeInteger ;
            owl:onProperty schema:name ],
        schema:Project ;
    skos:closeMatch frapo:Grant,
        <http://www.cidoc-crm.org/cidoc-crm/E7_Activity> ;
    skos:exactMatch <https://sshoc.eu/ontology/SHE3_SSH_Project> .

sioc:topic a owl:ObjectProperty ;
    rdfs:label "sioc:topic"@en ;
    rdfs:comment "A topic of interest, linking to the concept URI."@en,
        "A topic of interest, linking to the concept URI. Links to discipline terms."@en ;
    rdfs:subPropertyOf dcterms:subject .

schema:ContactPoint a owl:Class ;
    rdfs:label "schema:ContactPoint",
        "schema:ContactPoint"@en ;
    rdfs:comment "A contact point for a person or organization"@en,
        "A contact point for a person or organization."@en .

schema:DefinedTerm a owl:Class ;
    rdfs:label "schema:DefinedTerm"@en ;
    rdfs:comment "A word, name, acronym, phrase, etc. with a formal definition"@en ;
    rdfs:subClassOf [ a owl:Restriction ;
            owl:onProperty schema:name ;
            owl:someValuesFrom schema:Text ] .

schema:Language a owl:Class ;
    rdfs:label "schema:Language"@en ;
    rdfs:comment "Natural language such as Spanish, Tamil, or English."@en .

schema:datePublished a owl:DatatypeProperty ;
    rdfs:label "schema:datePublished",
        "schema:datePublished"@en ;
    rdfs:comment "Date of first broadcast/publication."@en,
        "Date of first publication"@en,
        "Date of first publication or broadcast"@en ;
    rdfs:range xsd:date .

schema:name a owl:DatatypeProperty ;
    rdfs:label "schema:name",
        "name"@en,
        "schema:name"@en ;
    rdfs:comment "The name of the item."@en ;
    rdfs:range xsd:string .

dcterms:isReferencedBy a owl:ObjectProperty ;
    rdfs:label "dcterms:isReferencedBy"@en ;
    rdfs:comment "A related resource that references, cites, or otherwise points to the described resource."@en,
        "A related resource that references, cites, or otherwise points to the multimedia object."@en .

schema:dateCreated a owl:DatatypeProperty ;
    rdfs:label "schema:dateCreated",
        "schema:dateCreated"@en ;
    rdfs:comment "The date on which the CreativeWork was created"@en,
        "The date on which the CreativeWork was created or the item was added to a DataFeed."@en ;
    rdfs:range xsd:date .

schema:dateModified a owl:DatatypeProperty ;
    rdfs:label "schema:dateModified",
        "schema:dateModified"@en ;
    rdfs:comment "The date on which the CreativeWork was most recently modified"@en,
        "The date on which the CreativeWork was most recently modified or when the item's entry was modified within a DataFeed."@en ;
    rdfs:range xsd:date .

datacite:usesIdentifierScheme a owl:ObjectProperty ;
    rdfs:label "datacite:usesIdentifierScheme"@en ;
    rdfs:comment "Links an identifier to its scheme"@en,
        "The reference identifier scheme used to identify the entity."@en ;
    rdfs:domain datacite:Identifier ;
    rdfs:range datacite:IdentifierScheme .

litre:hasLiteralValue a owl:DatatypeProperty ;
    rdfs:label "litre:hasLiteralValue"@en ;
    rdfs:comment "Associates an entity with a literal value representing its textual content."@en ;
    rdfs:range xsd:string .

skos:Concept a owl:Class ;
    rdfs:label "Concept"@en,
        "skos:Concept"@en ;
    rdfs:comment "A SKOS concept representing a term in a controlled vocabulary."@en .

datacite:IdentifierScheme a owl:Class ;
    rdfs:label "datacite:IdentifierScheme"@en ;
    rdfs:comment "A scheme that uniquely identifies entities of a particular type."@en .

datacite:hasIdentifier a owl:ObjectProperty ;
    rdfs:label "datacite:hasIdentifier",
        "datacite:hasIdentifier"@en ;
    rdfs:comment "Links entities to their identifiers"@en ;
    rdfs:range datacite:Identifier .

datacite:Identifier a owl:Class ;
    rdfs:label "datacite:Identifier"@en ;
    rdfs:comment "An identifier that uniquely identifies an entity according to some identification scheme."@en ;
    rdfs:subClassOf [ a owl:Restriction ;
            owl:onClass datacite:IdentifierScheme ;
            owl:onProperty datacite:usesIdentifierScheme ;
            owl:qualifiedCardinality "1"^^xsd:nonNegativeInteger ],
        [ a owl:Restriction ;
            owl:onDataRange xsd:string ;
            owl:onProperty litre:hasLiteralValue ;
            owl:qualifiedCardinality "1"^^xsd:nonNegativeInteger ] .

foaf:Organization a owl:Class ;
    rdfs:label "foaf:Organization"@en ;
    rdfs:comment "An organization."@en ;
    rdfs:subClassOf [ a owl:Restriction ;
            owl:onDataRange xsd:string ;
            owl:onProperty schema:name ;
            owl:qualifiedCardinality "1"^^xsd:nonNegativeInteger ],
        schema:Thing .

foaf:Person a owl:Class ;
    rdfs:label "foaf:Person"@en ;
    rdfs:comment "A person."@en ;
    rdfs:subClassOf [ a owl:Restriction ;
            owl:onDataRange xsd:string ;
            owl:onProperty schema:name ;
            owl:qualifiedCardinality "1"^^xsd:nonNegativeInteger ],
        schema:Thing ;
    owl:equivalentClass schema:Person .

