@prefix : <https://gotriple.eu/ontology/triple#> .
@prefix owl: <http://www.w3.org/2002/07/owl#> .
@prefix rdf: <http://www.w3.org/1999/02/22-rdf-syntax-ns#> .
@prefix xml: <http://www.w3.org/XML/1998/namespace> .
@prefix xsd: <http://www.w3.org/2001/XMLSchema#> .
@prefix rdfs: <http://www.w3.org/2000/01/rdf-schema#> .
@prefix schema: <http://schema.org/> .
@prefix triple: <https://gotriple.eu/ontology/triple#> .
@base <https://gotriple.eu/ontology/triple#> .

<https://gotriple.eu/ontology/triple> rdf:type owl:Ontology ;
                                       owl:versionIRI <https://gotriple.eu/ontology/triple/1.0.0> .

#################################################################
#    Classes
#################################################################

###  https://gotriple.eu/ontology/triple#SemanticArtefact
triple:SemanticArtefact rdf:type owl:Class ;
                        rdfs:subClassOf schema:CreativeWork ;
                        rdfs:label "Semantic Artefact"@en ;
                        rdfs:comment "A semantic artefact in the GoTriple platform, representing ontologies, vocabularies, taxonomies, thesauri, knowledge graphs, and other formal knowledge structures used in SSH research. It is a subclass of schema:CreativeWork."@en .


###  https://gotriple.eu/ontology/triple#Software
triple:Software rdf:type owl:Class ;
                rdfs:subClassOf schema:CreativeWork ;
                rdfs:label "Software"@en ;
                rdfs:comment "A software resource in the GoTriple platform, representing research software applications, tools, code repositories, libraries, scripts, algorithms, and computational workflows used in SSH research. It is a subclass of schema:CreativeWork."@en .


###  https://gotriple.eu/ontology/triple#Multimedia
triple:Multimedia rdf:type owl:Class ;
                  rdfs:subClassOf schema:CreativeWork ;
                  rdfs:label "Multimedia"@en ;
                  rdfs:comment "A multimedia resource in the GoTriple platform, representing audio-visual and interactive content such as audio recordings, video recordings, interviews, documentaries, lectures, and interactive media used in SSH research. It is a subclass of schema:CreativeWork."@en .


###  Generated by the OWL API (version 4.5.25.2023-02-15T19:15:49Z) https://github.com/owlcs/owlapi
