@prefix datacite: <http://purl.org/spar/datacite/> .
@prefix dcterms: <http://purl.org/dc/terms/> .
@prefix foaf: <http://xmlns.com/foaf/0.1/> .
@prefix litre: <http://purl.org/spar/literal/> .
@prefix owl: <http://www.w3.org/2002/07/owl#> .
@prefix rdf: <http://www.w3.org/1999/02/22-rdf-syntax-ns#> .
@prefix rdfs: <http://www.w3.org/2000/01/rdf-schema#> .
@prefix schema: <http://schema.org/> .
@prefix sioc: <http://rdfs.org/sioc/ns#> .
@prefix skos: <http://www.w3.org/2004/02/skos/core#> .
@prefix triple: <https://gotriple.eu/ontology/triple#> .
@prefix xsd: <http://www.w3.org/2001/XMLSchema#> .

datacite:hasIdentifierScheme a owl:ObjectProperty ;
    rdfs:label "datacite:hasIdentifierScheme"@en ;
    rdfs:comment "Links an identifier to its scheme"@en ;
    rdfs:domain datacite:Identifier .

schema:familyName a owl:DatatypeProperty ;
    rdfs:label "schema:familyName"@en ;
    rdfs:comment "Family name. In the U.S., the last name of a Person"@en ;
    rdfs:range xsd:string .

schema:geo a owl:ObjectProperty ;
    rdfs:label "schema:geo",
        "schema:geo"@en ;
    rdfs:comment "The geo coordinates of the place."@en ;
    rdfs:domain schema:Place ;
    rdfs:range schema:GeoShape .

schema:givenName a owl:DatatypeProperty ;
    rdfs:label "schema:givenName"@en ;
    rdfs:comment "Given name. In the U.S., the first name of a Person"@en ;
    rdfs:range xsd:string .

schema:license a owl:ObjectProperty ;
    rdfs:label "schema:license"@en ;
    rdfs:comment "The license under which the document is published. Links to license terms from controlled vocabulary. Official licenses reference: Creative Commons (https://creativecommons.org/licenses/), SPDX (https://spdx.org/licenses/)."@en .

skos:closeMatch a owl:ObjectProperty ;
    rdfs:label "skos:closeMatch"@en ;
    rdfs:comment "A SKOS property indicating that two concepts are sufficiently similar to be used interchangeably in some contexts."@en .

skos:definition a owl:AnnotationProperty ;
    rdfs:label "skos:definition"@en ;
    rdfs:comment "A SKOS annotation property providing a complete explanation of the intended meaning of a concept."@en .

skos:exactMatch a owl:ObjectProperty ;
    rdfs:label "skos:exactMatch"@en ;
    rdfs:comment "A SKOS property indicating that two concepts can be used interchangeably across all contexts."@en .

skos:inScheme a owl:ObjectProperty ;
    rdfs:label "skos:inScheme"@en ;
    rdfs:comment "A SKOS property linking a concept to the concept scheme it belongs to."@en .

<https://gotriple.eu/ontology/triple> a owl:Ontology ;
    rdfs:label "TRIPLE Ontology"@en ;
    dcterms:created "2025-10-06" ;
    dcterms:modified "2025-10-06" ;
    rdfs:comment "Comprehensive semantic representation of the GoTriple discovery platform's data model for Social Sciences and Humanities (SSH) research artifacts."@en ;
    owl:imports <https://gotriple.eu/ontology/triple/conditions_of_access#>,
        <https://gotriple.eu/ontology/triple/content_types#>,
        <https://gotriple.eu/ontology/triple/disciplines#>,
        <https://gotriple.eu/ontology/triple/licenses#> ;
    owl:versionIRI <https://gotriple.eu/ontology/triple/1.0.0> ;
    owl:versionInfo "1.0.0" .

triple:Dataset a owl:Class ;
    rdfs:label "Dataset"@en,
        "Dataset (Triple)"@en ;
    rdfs:comment "A collection of data organized for research purposes in the Social Sciences and Humanities domain."@en,
        "A dataset in the GoTriple platform, representing research data with specific metadata including spatial coverage, temporal coverage, and distribution information. It is a subclass of schema:Dataset."@en ;
    rdfs:subClassOf [ a owl:Restriction ;
            owl:allValuesFrom schema:Place ;
            owl:onProperty schema:spatialCoverage ],
        [ a owl:Restriction ;
            owl:allValuesFrom [ owl:unionOf ( foaf:Person foaf:Organization ) ] ;
            owl:onProperty schema:publisher ],
        [ a owl:Restriction ;
            owl:allValuesFrom [ owl:unionOf ( foaf:Person foaf:Organization ) ] ;
            owl:onProperty schema:provider ],
        [ a owl:Restriction ;
            owl:allValuesFrom owl:Thing ;
            owl:onProperty schema:funding ],
        [ a owl:Restriction ;
            owl:allValuesFrom owl:Thing ;
            owl:onProperty schema:contactPoint ],
        [ a owl:Restriction ;
            owl:allValuesFrom owl:Thing ;
            owl:onProperty schema:mentions ],
        [ a owl:Restriction ;
            owl:allValuesFrom schema:DefinedTerm ;
            owl:onProperty schema:keywords ],
        [ a owl:Restriction ;
            owl:allValuesFrom owl:Thing ;
            owl:onProperty sioc:topic ],
        [ a owl:Restriction ;
            owl:allValuesFrom owl:Thing ;
            owl:onProperty dcterms:isReferencedBy ],
        [ a owl:Restriction ;
            owl:allValuesFrom xsd:string ;
            owl:onProperty schema:temporalCoverage ],
        [ a owl:Restriction ;
            owl:allValuesFrom xsd:string ;
            owl:onProperty schema:encodingFormat ],
        [ a owl:Restriction ;
            owl:allValuesFrom xsd:string ;
            owl:onProperty schema:size ],
        [ a owl:Restriction ;
            owl:allValuesFrom xsd:string ;
            owl:onProperty schema:creativeWorkStatus ],
        [ a owl:Restriction ;
            owl:allValuesFrom datacite:Identifier ;
            owl:onProperty datacite:hasIdentifier ],
        [ a owl:Restriction ;
            owl:allValuesFrom rdf:langString ;
            owl:onProperty schema:headline ],
        [ a owl:Restriction ;
            owl:allValuesFrom [ owl:unionOf ( foaf:Person foaf:Organization ) ] ;
            owl:onProperty schema:author ],
        [ a owl:Restriction ;
            owl:allValuesFrom rdf:langString ;
            owl:onProperty schema:abstract ],
        [ a owl:Restriction ;
            owl:allValuesFrom xsd:string ;
            owl:onProperty schema:additionalType ],
        [ a owl:Restriction ;
            owl:allValuesFrom xsd:string ;
            owl:onProperty schema:knowsAbout ],
        [ a owl:Restriction ;
            owl:onProperty schema:inLanguage ;
            owl:someValuesFrom schema:Language ],
        [ a owl:Restriction ;
            owl:allValuesFrom xsd:date ;
            owl:onProperty schema:dateCreated ],
        [ a owl:Restriction ;
            owl:allValuesFrom xsd:date ;
            owl:onProperty schema:datePublished ],
        [ a owl:Restriction ;
            owl:allValuesFrom xsd:date ;
            owl:onProperty schema:dateModified ],
        [ a owl:Restriction ;
            owl:maxCardinality "1"^^xsd:nonNegativeInteger ;
            owl:onProperty schema:dateCreated ],
        [ a owl:Restriction ;
            owl:maxCardinality "1"^^xsd:nonNegativeInteger ;
            owl:onProperty schema:datePublished ],
        [ a owl:Restriction ;
            owl:maxCardinality "1"^^xsd:nonNegativeInteger ;
            owl:onProperty schema:dateModified ],
        [ a owl:Restriction ;
            owl:allValuesFrom xsd:string ;
            owl:onProperty schema:comment ],
        [ a owl:Restriction ;
            owl:onProperty sioc:topic ;
            owl:someValuesFrom skos:Concept ],
        [ a owl:Restriction ;
            owl:allValuesFrom [ owl:unionOf ( foaf:Person foaf:Organization ) ] ;
            owl:onProperty schema:contributor ],
        [ a owl:Restriction ;
            owl:allValuesFrom triple:Project ;
            owl:onProperty <http://purl.org/cerif/frapo/isOutputOf> ],
        [ a owl:Restriction ;
            owl:allValuesFrom schema:CreativeWork ;
            owl:onProperty dcterms:isReferencedBy ],
        schema:Dataset .

triple:MediaObject a owl:Class ;
    rdfs:label "Media Object"@en,
        "Media Object (Triple)"@en ;
    rdfs:comment "A media object such as an image, video, audio, or other multimedia content used in SSH research."@en,
        "A multimedia object in the GoTriple platform, representing various types of media files (audio, video, images) associated with scholarly works."@en ;
    rdfs:subClassOf [ a owl:Restriction ;
            owl:allValuesFrom [ owl:unionOf ( foaf:Person foaf:Organization ) ] ;
            owl:onProperty schema:publisher ],
        [ a owl:Restriction ;
            owl:allValuesFrom [ owl:unionOf ( foaf:Person foaf:Organization ) ] ;
            owl:onProperty schema:provider ],
        [ a owl:Restriction ;
            owl:allValuesFrom [ owl:unionOf ( foaf:Person foaf:Organization ) ] ;
            owl:onProperty schema:producer ],
        [ a owl:Restriction ;
            owl:allValuesFrom schema:Place ;
            owl:onProperty schema:spatialCoverage ],
        [ a owl:Restriction ;
            owl:allValuesFrom schema:DefinedTerm ;
            owl:onProperty schema:keywords ],
        [ a owl:Restriction ;
            owl:allValuesFrom rdf:langString ;
            owl:onProperty schema:headline ],
        [ a owl:Restriction ;
            owl:allValuesFrom rdf:langString ;
            owl:onProperty schema:abstract ],
        [ a owl:Restriction ;
            owl:allValuesFrom xsd:date ;
            owl:onProperty schema:dateCreated ],
        [ a owl:Restriction ;
            owl:allValuesFrom xsd:date ;
            owl:onProperty schema:datePublished ],
        [ a owl:Restriction ;
            owl:allValuesFrom xsd:date ;
            owl:onProperty schema:dateModified ],
        [ a owl:Restriction ;
            owl:maxCardinality "1"^^xsd:nonNegativeInteger ;
            owl:onProperty schema:dateCreated ],
        [ a owl:Restriction ;
            owl:allValuesFrom [ owl:unionOf ( foaf:Person foaf:Organization ) ] ;
            owl:onProperty schema:author ],
        [ a owl:Restriction ;
            owl:maxCardinality "1"^^xsd:nonNegativeInteger ;
            owl:onProperty schema:datePublished ],
        [ a owl:Restriction ;
            owl:maxCardinality "1"^^xsd:nonNegativeInteger ;
            owl:onProperty schema:dateModified ],
        [ a owl:Restriction ;
            owl:allValuesFrom xsd:string ;
            owl:onProperty schema:encodingFormat ],
        [ a owl:Restriction ;
            owl:allValuesFrom xsd:string ;
            owl:onProperty schema:duration ],
        [ a owl:Restriction ;
            owl:allValuesFrom xsd:string ;
            owl:onProperty schema:size ],
        [ a owl:Restriction ;
            owl:onProperty schema:inLanguage ;
            owl:someValuesFrom schema:Language ],
        [ a owl:Restriction ;
            owl:allValuesFrom xsd:string ;
            owl:onProperty schema:temporalCoverage ],
        [ a owl:Restriction ;
            owl:allValuesFrom xsd:string ;
            owl:onProperty schema:additionalType ],
        [ a owl:Restriction ;
            owl:allValuesFrom xsd:string ;
            owl:onProperty schema:knowsAbout ],
        [ a owl:Restriction ;
            owl:allValuesFrom owl:Thing ;
            owl:onProperty schema:mentions ],
        [ a owl:Restriction ;
            owl:allValuesFrom datacite:Identifier ;
            owl:onProperty datacite:hasIdentifier ],
        [ a owl:Restriction ;
            owl:onProperty sioc:topic ;
            owl:someValuesFrom skos:Concept ],
        [ a owl:Restriction ;
            owl:allValuesFrom [ owl:unionOf ( foaf:Person foaf:Organization ) ] ;
            owl:onProperty schema:contributor ],
        [ a owl:Restriction ;
            owl:allValuesFrom triple:Project ;
            owl:onProperty <http://purl.org/cerif/frapo/isOutputOf> ],
        [ a owl:Restriction ;
            owl:allValuesFrom schema:CreativeWork ;
            owl:onProperty dcterms:isReferencedBy ],
        schema:MediaObject .

triple:SemanticArtefact a owl:Class ;
    rdfs:label "Semantic Artefact"@en ;
    rdfs:comment "A semantic artefact in the context of GoTriple platform, representing formal knowledge representations such as ontologies, controlled vocabularies, and other semantic resources used in SSH research."@en ;
    rdfs:subClassOf [ a owl:Restriction ;
            owl:allValuesFrom triple:Project ;
            owl:onProperty <http://purl.org/cerif/frapo/isOutputOf> ],
        [ a owl:Restriction ;
            owl:allValuesFrom schema:CreativeWork ;
            owl:onProperty dcterms:isReferencedBy ],
        schema:CreativeWork,
        <https://w3id.org/mod#SemanticArtefact> .

triple:acc_embargoed-access a owl:NamedIndividual,
        skos:Concept ;
    rdfs:label "Embargoed Access"@en ;
    skos:definition "The resource is under embargo and will become openly accessible after a specified date"@en ;
    skos:exactMatch <https://vocabularies.coar-repositories.org/access_rights/c_f1cf/> ;
    skos:inScheme triple:conditions_of_access .

triple:acc_metadata-only-access a owl:NamedIndividual,
        skos:Concept ;
    rdfs:label "Metadata Only Access"@en ;
    skos:definition "Only metadata about the resource is accessible; the resource itself is not available"@en ;
    skos:exactMatch <https://vocabularies.coar-repositories.org/access_rights/c_14cb/> ;
    skos:inScheme triple:conditions_of_access .

triple:acc_open-access a owl:NamedIndividual,
        skos:Concept ;
    rdfs:label "Open Access"@en ;
    skos:definition "The resource is freely accessible to anyone without restrictions"@en ;
    skos:exactMatch <https://vocabularies.coar-repositories.org/access_rights/c_abf2/> ;
    skos:inScheme triple:conditions_of_access .

triple:acc_restricted-access a owl:NamedIndividual,
        skos:Concept ;
    rdfs:label "Restricted Access"@en ;
    skos:definition "The resource is accessible only under certain conditions or to specific users"@en ;
    skos:exactMatch <https://vocabularies.coar-repositories.org/access_rights/c_16ec/> ;
    skos:inScheme triple:conditions_of_access .

triple:disciplines a owl:NamedIndividual,
        skos:ConceptScheme ;
    rdfs:label "Disciplines"@en ;
    rdfs:comment "Controlled vocabulary of academic disciplines used in GoTriple"@en .

triple:doi a datacite:IdentifierScheme,
        owl:NamedIndividual ;
    rdfs:label "DOI"@en ;
    rdfs:comment "Digital Object Identifier - a persistent identifier for digital objects maintained by the International DOI Foundation."@en .

triple:full_text_url a datacite:IdentifierScheme,
        owl:NamedIndividual ;
    rdfs:label "Full Text URL"@en ;
    rdfs:comment "URL providing direct access to the full content of the document."@en .

triple:handle a datacite:IdentifierScheme,
        owl:NamedIndividual ;
    rdfs:label "Handle"@en ;
    rdfs:comment "Handle System - a persistent identifier infrastructure for managing digital objects."@en .

triple:internal_id a datacite:IdentifierScheme,
        owl:NamedIndividual ;
    rdfs:label "Internal ID"@en ;
    rdfs:comment "Internal identifier used within the GoTriple platform for document management."@en .

triple:isDiscarded a owl:DatatypeProperty ;
    rdfs:label "is discarded"@en ;
    rdfs:comment "A boolean flag indicating whether an entity (author or keyword) has been marked as discarded and should not be used for search/filtering."@en ;
    rdfs:range xsd:boolean .

triple:isbn a datacite:IdentifierScheme,
        owl:NamedIndividual ;
    rdfs:label "ISBN"@en ;
    rdfs:comment "International Standard Book Number - a numeric identifier for books and book-like products."@en .

triple:issn a datacite:IdentifierScheme,
        owl:NamedIndividual ;
    rdfs:label "ISSN"@en ;
    rdfs:comment "International Standard Serial Number - an eight-digit identifier for serial publications."@en .

triple:landing_page_url a datacite:IdentifierScheme,
        owl:NamedIndividual ;
    rdfs:label "Landing Page URL"@en ;
    rdfs:comment "URL of the landing page containing metadata and descriptive information about the document."@en .

triple:licenses a owl:NamedIndividual,
        skos:ConceptScheme ;
    rdfs:label "Licenses"@en ;
    rdfs:comment "Controlled vocabulary of licenses used in GoTriple"@en .

triple:original_id a datacite:IdentifierScheme,
        owl:NamedIndividual ;
    rdfs:label "Original ID"@en ;
    rdfs:comment "Original identifier from the source system where the document was harvested."@en .

triple:pid a datacite:IdentifierScheme,
        owl:NamedIndividual ;
    rdfs:label "PID"@en ;
    rdfs:comment "Persistent identifier generated and exposed externally by the GoTriple platform."@en .

triple:source_url a datacite:IdentifierScheme,
        owl:NamedIndividual ;
    rdfs:label "Source URL"@en ;
    rdfs:comment "URL of the original publication location or source repository."@en .

triple:typ_book-part a owl:NamedIndividual,
        skos:Concept ;
    rdfs:label "Book Part"@en ;
    skos:definition "A defined chapter or section of a book, usually with a separate title or number"@en ;
    skos:exactMatch <https://vocabularies.coar-repositories.org/resource_types/c_3248/> ;
    skos:inScheme triple:content_types .

datacite:usesIdentifierScheme a owl:ObjectProperty ;
    rdfs:label "datacite:usesIdentifierScheme"@en .

litre:hasLiteralValue a owl:DatatypeProperty .

schema:GeoShape a owl:Class ;
    rdfs:label "schema:GeoShape"@en ;
    rdfs:comment "The geographic shape of a place. A GeoShape can be described using several properties whose values are based on latitude/longitude pairs."@en .

schema:Grant a owl:Class ;
    rdfs:label "schema:Grant"@en ;
    rdfs:comment "A grant, typically financial or otherwise quantifiable, of resources"@en ;
    rdfs:subClassOf [ a owl:Restriction ;
            owl:allValuesFrom [ owl:unionOf ( foaf:Person foaf:Organization ) ] ;
            owl:onProperty schema:funder ],
        [ a owl:Restriction ;
            owl:allValuesFrom [ owl:unionOf ( foaf:Person foaf:Organization ) ] ;
            owl:onProperty schema:sponsor ] .

schema:MediaObject a owl:Class ;
    rdfs:label "schema:MediaObject"@en ;
    rdfs:comment "A media object, such as an image, video, or audio object embedded in a web page or a downloadable dataset. Note that a creative work may have many media objects associated with it on the same web page."@en .

schema:Project a owl:Class ;
    rdfs:label "schema:Project"@en ;
    rdfs:comment "An enterprise (potentially individual but typically collaborative), planned to achieve a particular aim."@en .

schema:Text a rdfs:Datatype .

schema:about a owl:ObjectProperty ;
    rdfs:label "schema:about"@en ;
    rdfs:comment "The subject matter of the content"@en .

schema:alternateName a owl:DatatypeProperty ;
    rdfs:label "schema:alternateName"@en ;
    rdfs:comment "An alias for the item"@en ;
    rdfs:range rdf:langString .

schema:comment a owl:DatatypeProperty ;
    rdfs:label "schema:comment"@en ;
    rdfs:comment "Comments, typically from users."@en .

schema:conditionsOfAccess a owl:ObjectProperty ;
    rdfs:label "schema:conditionsOfAccess"@en ;
    rdfs:comment "Conditions that affect the availability of, or method(s) of access to, an item."@en,
        "The conditions under which the document can be accessed. Links to access rights terms from controlled vocabulary. Official reference: COAR Access Rights Vocabulary (http://vocabularies.coar-repositories.org/access_rights/)."@en ;
    rdfs:range skos:Concept .

schema:contactPoint a owl:ObjectProperty ;
    rdfs:label "schema:contactPoint"@en ;
    rdfs:comment "A contact point for a person or organization."@en .

schema:creativeWorkStatus a owl:DatatypeProperty ;
    rdfs:label "schema:creativeWorkStatus"@en ;
    rdfs:comment "The status of a creative work in terms of its stage in a lifecycle."@en .

schema:description a owl:DatatypeProperty ;
    rdfs:label "schema:description"@en ;
    rdfs:comment "A description of the item"@en ;
    rdfs:range rdf:langString .

schema:duration a owl:DatatypeProperty ;
    rdfs:label "schema:duration"@en ;
    rdfs:comment "The duration of the item (movie, audio recording, event, etc.) in ISO 8601 duration format."@en .

schema:sponsor a owl:ObjectProperty ;
    rdfs:label "schema:sponsor"@en ;
    rdfs:comment "A person or organization that supports a thing through a pledge, promise, or financial contribution"@en .

foaf:Document a owl:Class ;
    rdfs:label "foaf:Document"@en .

foaf:OnlineAccount a owl:Class ;
    rdfs:label "foaf:OnlineAccount"@en ;
    rdfs:subClassOf [ a owl:Restriction ;
            owl:onClass datacite:Identifier ;
            owl:onProperty datacite:hasIdentifier ;
            owl:qualifiedCardinality "1"^^xsd:nonNegativeInteger ] .

foaf:account a owl:ObjectProperty ;
    rdfs:label "foaf:account"@en ;
    rdfs:comment "Indicates an account held by this agent"@en .

triple:Document a owl:Class ;
    rdfs:label "Document"@en,
        "Document (Triple)"@en ;
    rdfs:comment "A document in the GoTriple platform, representing scholarly publications and research outputs."@en,
        "A document in the GoTriple platform, representing scholarly publications, research datasets, and other SSH research artifacts. It is a subclass of both schema:CreativeWork and foaf:Document."@en ;
    rdfs:subClassOf [ a owl:Restriction ;
            owl:allValuesFrom triple:Profile ;
            owl:onProperty schema:author ],
        [ a owl:Restriction ;
            owl:onProperty schema:conditionsOfAccess ;
            owl:someValuesFrom skos:Concept ],
        [ a owl:Restriction ;
            owl:onProperty schema:keywords ;
            owl:someValuesFrom schema:DefinedTerm ],
        [ a owl:Restriction ;
            owl:onProperty schema:spatialCoverage ;
            owl:someValuesFrom schema:Place ],
        [ a owl:Restriction ;
            owl:onProperty schema:temporalCoverage ;
            owl:someValuesFrom xsd:string ],
        [ a owl:Restriction ;
            owl:onClass triple:Cluster ;
            owl:onProperty triple:inCluster ;
            owl:qualifiedCardinality "1"^^xsd:nonNegativeInteger ],
        [ a owl:Restriction ;
            owl:onProperty schema:additionalType ;
            owl:someValuesFrom skos:Concept ],
        [ a owl:Restriction ;
            owl:onProperty datacite:hasIdentifier ;
            owl:someValuesFrom datacite:Identifier ],
        [ a owl:Restriction ;
            owl:onProperty schema:inLanguage ;
            owl:someValuesFrom schema:Language ],
        [ a owl:Restriction ;
            owl:onProperty schema:headline ;
            owl:someValuesFrom rdf:langString ],
        [ a owl:Restriction ;
            owl:onProperty schema:abstract ;
            owl:someValuesFrom rdf:langString ],
        [ a owl:Restriction ;
            owl:onProperty schema:encodingFormat ;
            owl:someValuesFrom xsd:string ],
        [ a owl:Restriction ;
            owl:onProperty sioc:topic ;
            owl:someValuesFrom skos:Concept ],
        [ a owl:Restriction ;
            owl:allValuesFrom [ owl:unionOf ( foaf:Person foaf:Organization ) ] ;
            owl:onProperty schema:author ],
        [ a owl:Restriction ;
            owl:allValuesFrom [ owl:unionOf ( foaf:Person foaf:Organization ) ] ;
            owl:onProperty schema:contributor ],
        [ a owl:Restriction ;
            owl:allValuesFrom [ owl:unionOf ( foaf:Person foaf:Organization ) ] ;
            owl:maxCardinality 1 ;
            owl:onProperty schema:publisher ],
        [ a owl:Restriction ;
            owl:allValuesFrom [ owl:unionOf ( foaf:Person foaf:Organization ) ] ;
            owl:onProperty schema:producer ],
        [ a owl:Restriction ;
            owl:allValuesFrom [ owl:unionOf ( foaf:Person foaf:Organization ) ] ;
            owl:onProperty schema:funder ],
        [ a owl:Restriction ;
            owl:allValuesFrom [ owl:unionOf ( foaf:Person foaf:Organization ) ] ;
            owl:onProperty schema:provider ],
        [ a owl:Restriction ;
            owl:allValuesFrom [ owl:unionOf ( foaf:Person foaf:Organization ) ] ;
            owl:onProperty triple:aggregator ],
        [ a owl:Restriction ;
            owl:allValuesFrom [ owl:unionOf ( foaf:Person foaf:Organization ) ] ;
            owl:onProperty triple:primaryProducer ],
        [ a owl:Restriction ;
            owl:allValuesFrom triple:Project ;
            owl:onProperty <http://purl.org/cerif/frapo/isOutputOf> ],
        schema:CreativeWork,
        foaf:Document .

triple:aggregator a owl:ObjectProperty ;
    rdfs:label "aggregator"@en ;
    rdfs:comment "An aggregator that collates resources from different sources"@en ;
    rdfs:range [ owl:unionOf ( foaf:Person foaf:Organization ) ] ;
    rdfs:subPropertyOf schema:contributor .

triple:alsoKnownAs a owl:ObjectProperty ;
    rdfs:label "also known as"@en ;
    rdfs:comment "Links an ambiguous profile to the original profile"@en ;
    rdfs:domain triple:Profile ;
    rdfs:range triple:Profile .

triple:content_types a owl:NamedIndividual,
        skos:ConceptScheme ;
    rdfs:label "Content Types"@en ;
    rdfs:comment "Controlled vocabulary of content types used in GoTriple"@en .

triple:inCluster a owl:ObjectProperty ;
    rdfs:label "in cluster"@en ;
    rdfs:comment "Associates a document with its cluster (for deduplication purposes)."@en ;
    rdfs:domain triple:Document ;
    rdfs:range triple:Cluster .

triple:primaryProducer a owl:ObjectProperty ;
    rdfs:label "primary producer"@en ;
    rdfs:comment "The original source or creator of the resource"@en ;
    rdfs:range [ owl:unionOf ( foaf:Person foaf:Organization ) ] ;
    rdfs:subPropertyOf schema:producer .

schema:Thing a owl:Class ;
    rdfs:label "schema:Thing"@en .

schema:endDate a owl:DatatypeProperty ;
    rdfs:label "schema:endDate"@en ;
    rdfs:comment "The end date and time of the item"@en ;
    rdfs:range xsd:date .

schema:funder a owl:ObjectProperty ;
    rdfs:label "schema:funder"@en ;
    rdfs:comment "A person or organization that supports something through some kind of financial contribution"@en,
        "A person or organization that supports through funding"@en ;
    rdfs:range [ owl:unionOf ( foaf:Person foaf:Organization ) ] .

schema:funding a owl:ObjectProperty ;
    rdfs:label "schema:funding"@en ;
    rdfs:comment "A Grant that directly or indirectly provide funding or sponsorship for this item."@en,
        "A grant, typically financial or otherwise quantifiable, of resources"@en .

schema:knowsAbout a owl:DatatypeProperty ;
    rdfs:label "schema:knowsAbout"@en ;
    rdfs:comment "Of a Person, and less typically of an Organization, to indicate a topic that is known about."@en ;
    rdfs:range xsd:string .

schema:mentions a owl:ObjectProperty ;
    rdfs:label "schema:mentions"@en ;
    rdfs:comment "Indicates that the CreativeWork contains a reference to, but is not necessarily about a particular thing."@en ;
    rdfs:range owl:Thing .

schema:size a owl:DatatypeProperty ;
    rdfs:label "schema:size"@en ;
    rdfs:comment "A standardized size of a product or creative work, specified either through a simple textual string or a QuantitativeValue."@en,
        "A standardized size of a product or creative work."@en .

schema:startDate a owl:DatatypeProperty ;
    rdfs:label "schema:startDate"@en ;
    rdfs:comment "The start date and time of the item"@en ;
    rdfs:range xsd:date .

triple:Cluster a owl:Class ;
    rdfs:label "Cluster"@en ;
    rdfs:comment "A cluster groups multiple documents from different sources that represent the same scholarly work. Used for deduplication."@en ;
    rdfs:subClassOf [ a owl:Restriction ;
            owl:onClass datacite:Identifier ;
            owl:onProperty datacite:hasIdentifier ;
            owl:qualifiedCardinality "1"^^xsd:nonNegativeInteger ] .

schema:abstract a owl:DatatypeProperty ;
    rdfs:label "schema:abstract"@en ;
    rdfs:comment "An abstract is a short description that summarizes a CreativeWork."@en ;
    rdfs:range rdf:langString .

schema:additionalType a owl:DatatypeProperty,
        owl:ObjectProperty ;
    rdfs:label "schema:additionalType"@en ;
    rdfs:comment "An additional type for the item, typically used for adding more specific types from external vocabularies."@en,
        "An additional type for the item, typically used for adding more specific types from external vocabularies. Links to document type terms from controlled vocabulary. Official reference: COAR Resource Types (http://vocabularies.coar-repositories.org/resource_types/)."@en,
        "An additional type for the item, typically used for adding more specific types."@en,
        "An additional type for the item."@en ;
    rdfs:range xsd:string .

schema:encodingFormat a owl:DatatypeProperty ;
    rdfs:label "schema:encodingFormat"@en ;
    rdfs:comment "Media type typically expressed using a MIME format."@en .

schema:headline a owl:DatatypeProperty ;
    rdfs:label "schema:headline"@en ;
    rdfs:comment "Headline of the article."@en ;
    rdfs:range rdf:langString .

schema:inLanguage a owl:ObjectProperty ;
    rdfs:label "schema:inLanguage"@en ;
    rdfs:comment "The language of the content or performance or used in an action."@en ;
    rdfs:range schema:Language .

schema:producer a owl:ObjectProperty ;
    rdfs:label "schema:producer"@en ;
    rdfs:comment "The person or organization who produced the work"@en,
        "The person or organization who produced the work (e.g. music album, movie, tv/radio series etc.)."@en ;
    rdfs:range [ owl:unionOf ( foaf:Person foaf:Organization ) ] .

schema:provider a owl:ObjectProperty ;
    rdfs:label "schema:provider"@en ;
    rdfs:comment "The service provider, organization, or individual that provides the data"@en,
        "The service provider, service operator, or service performer."@en,
        "The service provider, service operator, or service performer; the goods producer."@en ;
    rdfs:range [ owl:unionOf ( foaf:Person foaf:Organization ) ] .

schema:publisher a owl:ObjectProperty ;
    rdfs:label "schema:publisher"@en ;
    rdfs:comment "The publisher of the creative work"@en,
        "The publisher of the creative work."@en ;
    rdfs:range [ owl:unionOf ( foaf:Person foaf:Organization ) ] .

schema:spatialCoverage a owl:ObjectProperty ;
    rdfs:label "schema:spatialCoverage",
        "schema:spatialCoverage"@en ;
    rdfs:comment "The spatialCoverage of a CreativeWork indicates the place(s) which are the focus of the content."@en ;
    rdfs:range schema:Place .

schema:temporalCoverage a owl:DatatypeProperty ;
    rdfs:label "schema:temporalCoverage",
        "schema:temporalCoverage"@en ;
    rdfs:comment "The temporalCoverage of a CreativeWork indicates the period that the content applies to."@en ;
    rdfs:range xsd:string .

<http://purl.org/cerif/frapo/isOutputOf> a owl:ObjectProperty ;
    rdfs:label "frapo:isOutputOf"@en ;
    rdfs:comment "Indicates that a research output is the result of a particular project."@en ;
    rdfs:range triple:Project .

dcterms:isReferencedBy a owl:ObjectProperty ;
    rdfs:label "dcterms:isReferencedBy"@en ;
    rdfs:comment "A related resource that references, cites, or otherwise points to the described resource."@en .

sioc:topic a owl:ObjectProperty ;
    rdfs:label "sioc:topic"@en ;
    rdfs:comment "A topic of interest, linking to the concept URI."@en,
        "A topic of interest, linking to the concept URI. The subject or topic of the document. Links to subject/discipline terms from controlled vocabulary. Official references: UNESCO Thesaurus (https://vocabularies.unesco.org/), Library of Congress Subject Headings (https://id.loc.gov/authorities/subjects/)."@en .

schema:Language a owl:Class ;
    rdfs:label "schema:Language"@en ;
    rdfs:comment "Natural language such as Spanish, Tamil, or English."@en .

schema:author a owl:ObjectProperty ;
    rdfs:label "schema:author"@en ;
    rdfs:comment "The author of this content"@en,
        "The author of this content or rating."@en ;
    rdfs:range [ owl:unionOf ( foaf:Person foaf:Organization ) ] ;
    rdfs:subPropertyOf schema:creator .

schema:contributor a owl:ObjectProperty ;
    rdfs:label "schema:contributor"@en ;
    rdfs:comment "A secondary contributor to the CreativeWork"@en,
        "A secondary contributor to the CreativeWork or Event."@en,
        "A secondary contributor to the creative work or event."@en ;
    rdfs:range [ owl:unionOf ( foaf:Person foaf:Organization ) ] .

schema:dateCreated a owl:DatatypeProperty ;
    rdfs:label "schema:dateCreated"@en ;
    rdfs:comment "The date on which the CreativeWork was created or the item was added to a DataFeed."@en .

schema:dateModified a owl:DatatypeProperty ;
    rdfs:label "schema:dateModified"@en ;
    rdfs:comment "The date on which the CreativeWork was most recently modified or when the item's entry was modified within a DataFeed."@en .

schema:datePublished a owl:DatatypeProperty ;
    rdfs:label "schema:datePublished"@en ;
    rdfs:comment "Date of first broadcast/publication."@en,
        "Date of first publication or broadcast"@en ;
    rdfs:range xsd:date .

schema:keywords a owl:ObjectProperty ;
    rdfs:label "schema:keywords",
        "schema:keywords"@en ;
    rdfs:comment "Keywords or tags used to describe this content"@en,
        "Keywords or tags used to describe this content."@en ;
    rdfs:range schema:DefinedTerm .

skos:ConceptScheme a owl:Class ;
    rdfs:label "skos:ConceptScheme"@en ;
    rdfs:comment "A SKOS concept scheme representing a controlled vocabulary (e.g., licenses, document types, disciplines)."@en .

triple:Profile a owl:Class ;
    rdfs:label "profile"@en ;
    rdfs:comment "An author profile representing a person in the GoTriple system. Can be claimed or unclaimed."@en ;
    rdfs:subClassOf [ a owl:Restriction ;
            owl:maxCardinality "1"^^xsd:nonNegativeInteger ;
            owl:onClass foaf:OnlineAccount ;
            owl:onProperty foaf:account ],
        [ a owl:Restriction ;
            owl:maxCardinality "1"^^xsd:nonNegativeInteger ;
            owl:onClass triple:Profile ;
            owl:onProperty triple:alsoKnownAs ],
        foaf:Person .

triple:conditions_of_access a owl:NamedIndividual,
        skos:ConceptScheme ;
    rdfs:label "Conditions of Access"@en ;
    rdfs:comment "Controlled vocabulary of access conditions aligned with COAR Access Rights Vocabulary"@en,
        "Controlled vocabulary of access conditions used in GoTriple"@en .

schema:CreativeWork a owl:Class ;
    rdfs:label "schema:CreativeWork"@en .

schema:DefinedTerm a owl:Class ;
    rdfs:label "schema:DefinedTerm"@en ;
    rdfs:comment "A word, name, acronym, phrase, etc. with a formal definition"@en ;
    rdfs:subClassOf [ a owl:Restriction ;
            owl:onProperty schema:name ;
            owl:someValuesFrom schema:Text ] .

schema:Place a owl:Class ;
    rdfs:label "schema:Place"@en ;
    rdfs:comment "Entities that have a somewhat fixed, physical extension."@en ;
    rdfs:subClassOf [ a owl:Restriction ;
            owl:onProperty schema:name ;
            owl:someValuesFrom xsd:string ] .

schema:name a owl:DatatypeProperty ;
    rdfs:label "schema:name",
        "schema:name"@en ;
    rdfs:comment "The name of the item."@en ;
    rdfs:range xsd:string .

triple:Project a owl:Class ;
    rdfs:label "Project"@en,
        "Project (Triple)"@en ;
    rdfs:comment "A research project in the Social Sciences and Humanities domain integrated into the GoTriple platform."@en,
        "A research project in the Social Sciences and Humanities domain integrated into the GoTriple platform. It is a subclass of schema:Project."@en ;
    rdfs:subClassOf [ a owl:Restriction ;
            owl:allValuesFrom datacite:Identifier ;
            owl:onProperty datacite:hasIdentifier ],
        [ a owl:Restriction ;
            owl:maxCardinality "1"^^xsd:nonNegativeInteger ;
            owl:onProperty schema:startDate ],
        [ a owl:Restriction ;
            owl:allValuesFrom xsd:date ;
            owl:onProperty schema:startDate ],
        [ a owl:Restriction ;
            owl:allValuesFrom xsd:date ;
            owl:onProperty schema:endDate ],
        [ a owl:Restriction ;
            owl:maxCardinality "1"^^xsd:nonNegativeInteger ;
            owl:onProperty schema:endDate ],
        [ a owl:Restriction ;
            owl:allValuesFrom schema:Grant ;
            owl:onProperty schema:funding ],
        [ a owl:Restriction ;
            owl:allValuesFrom skos:Concept ;
            owl:onProperty schema:about ],
        [ a owl:Restriction ;
            owl:allValuesFrom schema:DefinedTerm ;
            owl:onProperty schema:keywords ],
        [ a owl:Restriction ;
            owl:allValuesFrom rdf:langString ;
            owl:onProperty schema:description ],
        [ a owl:Restriction ;
            owl:allValuesFrom rdf:langString ;
            owl:onProperty schema:alternateName ],
        [ a owl:Restriction ;
            owl:minCardinality "1"^^xsd:nonNegativeInteger ;
            owl:onProperty schema:name ],
        schema:Project .

datacite:hasIdentifier a owl:ObjectProperty ;
    rdfs:label "datacite:hasIdentifier"@en ;
    rdfs:comment "Links entities to their identifiers"@en ;
    rdfs:range datacite:Identifier .

datacite:Identifier a owl:Class ;
    rdfs:label "datacite:Identifier"@en ;
    rdfs:comment "An identifier that uniquely identifies an entity according to some identification scheme."@en ;
    rdfs:subClassOf [ a owl:Restriction ;
            owl:onClass datacite:IdentifierScheme ;
            owl:onProperty datacite:usesIdentifierScheme ;
            owl:qualifiedCardinality "1"^^xsd:nonNegativeInteger ],
        [ a owl:Restriction ;
            owl:onDataRange xsd:string ;
            owl:onProperty litre:hasLiteralValue ;
            owl:qualifiedCardinality "1"^^xsd:nonNegativeInteger ] .

datacite:IdentifierScheme a owl:Class ;
    rdfs:label "datacite:IdentifierScheme"@en ;
    rdfs:comment "A scheme that uniquely identifies entities of a particular type."@en .

skos:Concept a owl:Class ;
    rdfs:label "skos:Concept"@en ;
    rdfs:comment "A SKOS concept representing a term in a controlled vocabulary."@en .

foaf:Organization a owl:Class ;
    rdfs:label "foaf:Organization"@en ;
    rdfs:comment "An organization."@en ;
    rdfs:subClassOf [ a owl:Restriction ;
            owl:onDataRange xsd:string ;
            owl:onProperty schema:name ;
            owl:qualifiedCardinality "1"^^xsd:nonNegativeInteger ],
        schema:Thing .

foaf:Person a owl:Class ;
    rdfs:label "foaf:Person"@en ;
    rdfs:comment "A person."@en ;
    rdfs:subClassOf [ a owl:Restriction ;
            owl:onDataRange xsd:string ;
            owl:onProperty schema:name ;
            owl:qualifiedCardinality "1"^^xsd:nonNegativeInteger ],
        schema:Thing ;
    owl:equivalentClass schema:Person .

