@prefix : <https://gotriple.eu/ontology/triple#> .
@prefix owl: <http://www.w3.org/2002/07/owl#> .
@prefix rdf: <http://www.w3.org/1999/02/22-rdf-syntax-ns#> .
@prefix xml: <http://www.w3.org/XML/1998/namespace> .
@prefix xsd: <http://www.w3.org/2001/XMLSchema#> .
@prefix rdfs: <http://www.w3.org/2000/01/rdf-schema#> .
@prefix skos: <http://www.w3.org/2004/02/skos/core#> .
@prefix schema: <http://schema.org/> .
@prefix triple: <https://gotriple.eu/ontology/triple#> .
@prefix foaf: <http://xmlns.com/foaf/0.1/> .
@prefix dc: <http://purl.org/dc/elements/1.1/> .
@prefix dcterms: <http://purl.org/dc/terms/> .
@prefix datacite: <http://purl.org/spar/datacite/> .
@prefix litre: <http://purl.org/spar/literal/> .
@base <https://gotriple.eu/ontology/triple#> .

<https://gotriple.eu/ontology/triple> rdf:type owl:Ontology ;
                                       owl:versionIRI <https://gotriple.eu/ontology/triple/1.0.0> .

#################################################################
#    Object Properties
#################################################################

###  http://schema.org/contactPoint
schema:contactPoint rdf:type owl:ObjectProperty ;
                   rdfs:label "schema:contactPoint" ;
                   rdfs:comment "A contact point for a person or organization"@en ;
                   rdfs:domain triple:SemanticArtefact ;
                   rdfs:range schema:ContactPoint .

###  http://schema.org/creativeWorkStatus
schema:creativeWorkStatus rdf:type owl:ObjectProperty ;
                         rdfs:label "schema:creativeWorkStatus" ;
                         rdfs:comment "The status of a creative work in terms of its stage in a lifecycle"@en ;
                         rdfs:domain triple:SemanticArtefact ;
                         rdfs:range skos:Concept .

###  http://schema.org/keywords
schema:keywords rdf:type owl:ObjectProperty ;
               rdfs:label "schema:keywords" ;
               rdfs:comment "Keywords or tags used to describe the semantic artifact content"@en ;
               rdfs:domain triple:SemanticArtefact ;
               rdfs:range schema:DefinedTerm .

###  http://purl.org/dc/terms/isReferencedBy
dcterms:isReferencedBy rdf:type owl:ObjectProperty ;
                      rdfs:label "dcterms:isReferencedBy" ;
                      rdfs:comment "A related resource that references, cites, or otherwise points to the semantic artifact"@en ;
                      rdfs:domain triple:SemanticArtefact ;
                      rdfs:range triple:Document .

###  http://purl.org/spar/datacite/hasIdentifier
datacite:hasIdentifier rdf:type owl:ObjectProperty ;
                       rdfs:label "datacite:hasIdentifier" ;
                       rdfs:comment "Links the semantic artifact to its identifiers"@en ;
                       rdfs:domain triple:SemanticArtefact ;
                       rdfs:range datacite:Identifier .

###  http://schema.org/mainEntityOfPage
schema:mainEntityOfPage rdf:type owl:ObjectProperty ;
                        rdfs:label "schema:mainEntityOfPage" ;
                        rdfs:comment "Indicates a page (or other CreativeWork) for which this semantic artifact is the main entity being described (landing page)"@en ;
                        rdfs:domain triple:SemanticArtefact ;
                        rdfs:range foaf:Document .

#################################################################
#    Data Properties
#################################################################

###  http://schema.org/abstract
schema:abstract rdf:type owl:DatatypeProperty ;
               rdfs:label "schema:abstract" ;
               rdfs:comment "An abstract of the semantic artefact"@en ;
               rdfs:domain triple:SemanticArtefact ;
               rdfs:range rdf:langString .

###  http://schema.org/headline
schema:headline rdf:type owl:DatatypeProperty ;
               rdfs:label "schema:headline" ;
               rdfs:comment "The title or headline of the semantic artefact"@en ;
               rdfs:domain triple:SemanticArtefact ;
               rdfs:range rdf:langString .

###  http://schema.org/datePublished
schema:datePublished rdf:type owl:DatatypeProperty ;
                    rdfs:label "schema:datePublished" ;
                    rdfs:comment "Date of first publication of the semantic artefact"@en ;
                    rdfs:domain triple:SemanticArtefact ;
                    rdfs:range xsd:date .

###  http://schema.org/dateModified
schema:dateModified rdf:type owl:DatatypeProperty ;
                   rdfs:label "schema:dateModified" ;
                   rdfs:comment "The date on which the semantic artefact was most recently modified"@en ;
                   rdfs:domain triple:SemanticArtefact ;
                   rdfs:range xsd:date .

###  http://schema.org/version
schema:version rdf:type owl:DatatypeProperty ;
              rdfs:label "schema:version" ;
              rdfs:comment "The version of the semantic artefact"@en ;
              rdfs:domain triple:SemanticArtefact ;
              rdfs:range xsd:string .

###  http://schema.org/fileFormat
schema:fileFormat rdf:type owl:DatatypeProperty ;
                 rdfs:label "schema:fileFormat" ;
                 rdfs:comment "Media type, typically MIME format of the file (e.g., application/rdf+xml, text/turtle, application/zip)"@en ;
                 rdfs:domain triple:SemanticArtefact ;
                 rdfs:range xsd:string .

###  http://schema.org/encodingFormat
schema:encodingFormat rdf:type owl:DatatypeProperty ;
                     rdfs:label "schema:encodingFormat" ;
                     rdfs:comment "The representation technique or methodology used (e.g., OWL ontology, SKOS vocabulary, XML schema)"@en ;
                     rdfs:domain triple:SemanticArtefact ;
                     rdfs:range xsd:string .

###  http://schema.org/identifier
schema:identifier rdf:type owl:DatatypeProperty ;
                 rdfs:label "schema:identifier" ;
                 rdfs:comment "The identifier property represents any kind of identifier for the semantic artifact (local identifier, URI)"@en ;
                 rdfs:domain triple:SemanticArtefact ;
                 rdfs:range xsd:string .

###  http://schema.org/url
schema:url rdf:type owl:DatatypeProperty ;
          rdfs:label "schema:url" ;
          rdfs:comment "URL to access the semantic artifact"@en ;
          rdfs:domain triple:SemanticArtefact ;
          rdfs:range xsd:anyURI .

###  http://schema.org/isBasedOnUrl
schema:isBasedOnUrl rdf:type owl:DatatypeProperty ;
                   rdfs:label "schema:isBasedOnUrl" ;
                   rdfs:comment "A resource URL from which this semantic artifact is derived or from which it is a modification or adaptation"@en ;
                   rdfs:domain triple:SemanticArtefact ;
                   rdfs:range xsd:anyURI .

#################################################################
#    Classes
#################################################################

###  http://schema.org/ContactPoint
schema:ContactPoint rdf:type owl:Class ;
                   rdfs:label "schema:ContactPoint" ;
                   rdfs:comment "A contact point for a person or organization"@en .

###  http://purl.org/spar/datacite/Identifier
datacite:Identifier rdf:type owl:Class ;
                   rdfs:label "datacite:Identifier" ;
                   rdfs:comment "An identifier for a semantic artifact"@en .

###  http://purl.org/spar/datacite/IdentifierScheme
datacite:IdentifierScheme rdf:type owl:Class ;
                         rdfs:label "datacite:IdentifierScheme" ;
                         rdfs:comment "A scheme that defines the syntax and semantics of identifiers"@en .

###  https://gotriple.eu/ontology/triple#SemanticArtefact
triple:SemanticArtefact rdf:type owl:Class ;
                       rdfs:label "Semantic Artefact" ;
                       rdfs:comment "A semantic artefact such as an ontology, vocabulary, taxonomy, or concept scheme"@en ;
                       rdfs:subClassOf triple:Document ,
                                      [ rdf:type owl:Restriction ;
                                        owl:onProperty schema:headline ;
                                        owl:someValuesFrom rdf:langString
                                      ] ,
                                      [ rdf:type owl:Restriction ;
                                        owl:onProperty schema:abstract ;
                                        owl:someValuesFrom rdf:langString
                                      ] ,
                                      [ rdf:type owl:Restriction ;
                                        owl:onProperty schema:contributor ;
                                        owl:allValuesFrom [ owl:unionOf ( foaf:Person foaf:Organization ) ]
                                      ] ,
                                      [ rdf:type owl:Restriction ;
                                        owl:onProperty schema:inLanguage ;
                                        owl:someValuesFrom schema:Language
                                      ] ,
                                      [ rdf:type owl:Restriction ;
                                        owl:onProperty schema:datePublished ;
                                        owl:maxCardinality "1"^^xsd:nonNegativeInteger
                                      ] ,
                                      [ rdf:type owl:Restriction ;
                                        owl:onProperty schema:dateModified ;
                                        owl:maxCardinality "1"^^xsd:nonNegativeInteger
                                      ] ,
                                      [ rdf:type owl:Restriction ;
                                        owl:onProperty schema:version ;
                                        owl:maxCardinality "1"^^xsd:nonNegativeInteger
                                      ] ,
                                      [ rdf:type owl:Restriction ;
                                        owl:onProperty schema:publisher ;
                                        owl:allValuesFrom [ owl:unionOf ( foaf:Person foaf:Organization ) ]
                                      ] ,
                                      [ rdf:type owl:Restriction ;
                                        owl:onProperty triple:aggregator ;
                                        owl:allValuesFrom [ owl:unionOf ( foaf:Person foaf:Organization ) ]
                                      ] ,
                                      [ rdf:type owl:Restriction ;
                                        owl:onProperty schema:fileFormat ;
                                        owl:someValuesFrom xsd:string
                                      ] ,
                                      [ rdf:type owl:Restriction ;
                                        owl:onProperty schema:encodingFormat ;
                                        owl:someValuesFrom xsd:string
                                      ] ,
                                      [ rdf:type owl:Restriction ;
                                        owl:onProperty schema:contactPoint ;
                                        owl:allValuesFrom schema:ContactPoint
                                      ] ,
                                      [ rdf:type owl:Restriction ;
                                        owl:onProperty schema:creativeWorkStatus ;
                                        owl:maxCardinality "1"^^xsd:nonNegativeInteger
                                      ] ,
                                      [ rdf:type owl:Restriction ;
                                        owl:onProperty schema:keywords ;
                                        owl:allValuesFrom schema:DefinedTerm
                                      ] ,
                                      [ rdf:type owl:Restriction ;
                                        owl:onProperty dcterms:isReferencedBy ;
                                        owl:allValuesFrom triple:Document
                                      ] ,
                                      [ rdf:type owl:Restriction ;
                                        owl:onProperty datacite:hasIdentifier ;
                                        owl:allValuesFrom datacite:Identifier
                                      ] ,
                                      [ rdf:type owl:Restriction ;
                                        owl:onProperty schema:mainEntityOfPage ;
                                        owl:allValuesFrom foaf:Document
                                      ] ,
                                      [ rdf:type owl:Restriction ;
                                        owl:onProperty schema:identifier ;
                                        owl:allValuesFrom xsd:string
                                      ] ,
                                      [ rdf:type owl:Restriction ;
                                        owl:onProperty schema:url ;
                                        owl:allValuesFrom xsd:anyURI
                                      ] ,
                                      [ rdf:type owl:Restriction ;
                                        owl:onProperty schema:isBasedOnUrl ;
                                        owl:allValuesFrom xsd:anyURI
                                      ] .


#################################################################
#    Individuals
#################################################################

###  https://gotriple.eu/ontology/triple#doi
triple:doi rdf:type owl:NamedIndividual ,
                   datacite:IdentifierScheme ;
          rdfs:label "DOI" ;
          rdfs:comment "Digital Object Identifier - a persistent identifier for digital objects maintained by the International DOI Foundation"@en .

###  https://gotriple.eu/ontology/triple#handle
triple:handle rdf:type owl:NamedIndividual ,
                      datacite:IdentifierScheme ;
             rdfs:label "Handle" ;
             rdfs:comment "Handle System - a persistent identifier infrastructure for managing digital objects"@en .

###  https://gotriple.eu/ontology/triple#uri
triple:uri rdf:type owl:NamedIndividual ,
                   datacite:IdentifierScheme ;
          rdfs:label "URI" ;
          rdfs:comment "Uniform Resource Identifier - a string of characters that unambiguously identifies a particular resource"@en .
