@prefix : <https://gotriple.eu/ontology/triple#> .
@prefix owl: <http://www.w3.org/2002/07/owl#> .
@prefix rdf: <http://www.w3.org/1999/02/22-rdf-syntax-ns#> .
@prefix xml: <http://www.w3.org/XML/1998/namespace> .
@prefix xsd: <http://www.w3.org/2001/XMLSchema#> .
@prefix rdfs: <http://www.w3.org/2000/01/rdf-schema#> .
@prefix skos: <http://www.w3.org/2004/02/skos/core#> .
@prefix schema: <http://schema.org/> .
@prefix triple: <https://gotriple.eu/ontology/triple#> .
@prefix foaf: <http://xmlns.com/foaf/0.1/> .
@prefix dc: <http://purl.org/dc/elements/1.1/> .
@prefix dcterms: <http://purl.org/dc/terms/> .
@prefix datacite: <http://purl.org/spar/datacite/> .
@prefix litre: <http://purl.org/spar/literal/> .
@base <https://gotriple.eu/ontology/triple#> .

<https://gotriple.eu/ontology/triple> rdf:type owl:Ontology ;
                                       owl:versionIRI <https://gotriple.eu/ontology/triple/1.0.0> .

#################################################################
#    Object Properties
#################################################################

###  http://schema.org/spatialCoverage
schema:spatialCoverage rdf:type owl:ObjectProperty ;
                       rdfs:label "schema:spatialCoverage"@en ;
                       rdfs:comment "The spatialCoverage of a CreativeWork indicates the place(s) which are the focus of the content."@en ;
                       rdfs:range schema:Place .

###  http://schema.org/geo
schema:geo rdf:type owl:ObjectProperty ;
           rdfs:label "schema:geo"@en ;
           rdfs:comment "The geo coordinates of the place."@en ;
           rdfs:domain schema:Place ;
           rdfs:range schema:GeoShape .

###  http://schema.org/author
schema:author rdf:type owl:ObjectProperty ;
              rdfs:label "schema:author"@en ;
              rdfs:comment "The author of this content."@en ;
              rdfs:range [ owl:unionOf ( foaf:Person foaf:Organization ) ] .

###  http://schema.org/contributor
schema:contributor rdf:type owl:ObjectProperty ;
                   rdfs:label "schema:contributor"@en ;
                   rdfs:comment "A secondary contributor to the CreativeWork."@en ;
                   rdfs:range [ owl:unionOf ( foaf:Person foaf:Organization ) ] .

###  http://schema.org/publisher
schema:publisher rdf:type owl:ObjectProperty ;
                 rdfs:label "schema:publisher"@en ;
                 rdfs:comment "The publisher of the creative work."@en ;
                 rdfs:range [ owl:unionOf ( foaf:Person foaf:Organization ) ] .

###  http://schema.org/contactPoint
schema:contactPoint rdf:type owl:ObjectProperty ;
                   rdfs:label "schema:contactPoint" ;
                   rdfs:comment "A contact point for a person or organization"@en ;
                   rdfs:domain triple:SemanticArtefact ;
                   rdfs:range schema:ContactPoint .

###  http://schema.org/creativeWorkStatus
schema:creativeWorkStatus rdf:type owl:ObjectProperty ;
                         rdfs:label "schema:creativeWorkStatus" ;
                         rdfs:comment "The status of a creative work in terms of its stage in a lifecycle"@en ;
                         rdfs:domain triple:SemanticArtefact ;
                         rdfs:range skos:Concept .

###  http://schema.org/keywords
schema:keywords rdf:type owl:ObjectProperty ;
               rdfs:label "schema:keywords" ;
               rdfs:comment "Keywords or tags used to describe the semantic artifact content"@en ;
               rdfs:domain triple:SemanticArtefact ;
               rdfs:range schema:DefinedTerm .

###  http://purl.org/dc/terms/isReferencedBy
dcterms:isReferencedBy rdf:type owl:ObjectProperty ;
                      rdfs:label "dcterms:isReferencedBy" ;
                      rdfs:comment "A related resource that references, cites, or otherwise points to the semantic artifact"@en ;
                      rdfs:domain triple:SemanticArtefact ;
                      rdfs:range triple:Document .

###  http://purl.org/spar/datacite/hasIdentifier
datacite:hasIdentifier rdf:type owl:ObjectProperty ;
                       rdfs:label "datacite:hasIdentifier" ;
                       rdfs:comment "Links entities to their identifiers"@en ;
                       rdfs:range datacite:Identifier .


#################################################################
#    Data Properties
#################################################################

###  http://schema.org/name
schema:name rdf:type owl:DatatypeProperty ;
            rdfs:label "schema:name"@en ;
            rdfs:comment "The name of the item."@en ;
            rdfs:range xsd:string .

###  http://schema.org/abstract
schema:abstract rdf:type owl:DatatypeProperty ;
               rdfs:label "schema:abstract" ;
               rdfs:comment "An abstract of the semantic artefact"@en ;
               rdfs:domain triple:SemanticArtefact ;
               rdfs:range rdf:langString .

###  http://schema.org/headline
schema:headline rdf:type owl:DatatypeProperty ;
               rdfs:label "schema:headline" ;
               rdfs:comment "The title or headline of the semantic artefact"@en ;
               rdfs:domain triple:SemanticArtefact ;
               rdfs:range rdf:langString .

###  http://schema.org/datePublished
schema:datePublished rdf:type owl:DatatypeProperty ;
                    rdfs:label "schema:datePublished" ;
                    rdfs:comment "Date of first publication of the semantic artefact"@en ;
                    rdfs:domain triple:SemanticArtefact ;
                    rdfs:range xsd:date .

###  http://schema.org/dateModified
schema:dateModified rdf:type owl:DatatypeProperty ;
                   rdfs:label "schema:dateModified" ;
                   rdfs:comment "The date on which the semantic artefact was most recently modified"@en ;
                   rdfs:domain triple:SemanticArtefact ;
                   rdfs:range xsd:date .

###  http://schema.org/version
schema:version rdf:type owl:DatatypeProperty ;
              rdfs:label "schema:version" ;
              rdfs:comment "The version of the semantic artefact"@en ;
              rdfs:domain triple:SemanticArtefact ;
              rdfs:range xsd:string .

###  http://schema.org/fileFormat
schema:fileFormat rdf:type owl:DatatypeProperty ;
                 rdfs:label "schema:fileFormat" ;
                 rdfs:comment "Media type, typically MIME format of the file (e.g., application/rdf+xml, text/turtle, application/zip)"@en ;
                 rdfs:domain triple:SemanticArtefact ;
                 rdfs:range xsd:string .

###  http://schema.org/encodingFormat
schema:encodingFormat rdf:type owl:DatatypeProperty ;
                     rdfs:label "schema:encodingFormat" ;
                     rdfs:comment "The representation technique or methodology used (e.g., OWL ontology, SKOS vocabulary, XML schema)"@en ;
                     rdfs:domain triple:SemanticArtefact ;
                     rdfs:range xsd:string .




#################################################################
#    Classes
#################################################################

###  http://schema.org/Place
schema:Place rdf:type owl:Class ;
             rdfs:label "schema:Place"@en ;
             rdfs:comment "Entities that have a somewhat fixed, physical extension."@en ;
             rdfs:subClassOf [ rdf:type owl:Restriction ;
                              owl:onProperty schema:name ;
                              owl:someValuesFrom xsd:string ] .

###  http://schema.org/GeoShape
schema:GeoShape rdf:type owl:Class ;
                rdfs:label "schema:GeoShape"@en ;
                rdfs:comment "The geographic shape of a place. A GeoShape can be described using several properties whose values are based on latitude/longitude pairs."@en .

###  http://schema.org/ContactPoint
schema:ContactPoint rdf:type owl:Class ;
                   rdfs:label "schema:ContactPoint" ;
                   rdfs:comment "A contact point for a person or organization"@en .

###  http://xmlns.com/foaf/0.1/Person
foaf:Person rdf:type owl:Class ;
            rdfs:label "foaf:Person"@en ;
            rdfs:comment "A person."@en .

###  http://xmlns.com/foaf/0.1/Organization
foaf:Organization rdf:type owl:Class ;
                  rdfs:label "foaf:Organization"@en ;
                  rdfs:comment "An organization."@en .

###  http://purl.org/spar/datacite/Identifier
datacite:Identifier rdf:type owl:Class ;
                   rdfs:label "datacite:Identifier" ;
                   rdfs:comment "An identifier for a semantic artifact"@en .

###  http://purl.org/spar/datacite/IdentifierScheme
datacite:IdentifierScheme rdf:type owl:Class ;
                         rdfs:label "datacite:IdentifierScheme" ;
                         rdfs:comment "A scheme that defines the syntax and semantics of identifiers"@en .

###  https://gotriple.eu/ontology/triple#SemanticArtefact
triple:SemanticArtefact rdf:type owl:Class ;
                       rdfs:label "Semantic Artefact" ;
                       rdfs:comment "A semantic artefact such as an ontology, vocabulary, taxonomy, or concept scheme"@en ;
                       rdfs:subClassOf triple:Document ,
                                      [ rdf:type owl:Restriction ;
                                        owl:onProperty schema:headline ;
                                        owl:someValuesFrom rdf:langString
                                      ] ,
                                      [ rdf:type owl:Restriction ;
                                        owl:onProperty schema:abstract ;
                                        owl:someValuesFrom rdf:langString
                                      ] ,
                                      [ rdf:type owl:Restriction ;
                                        owl:onProperty schema:contributor ;
                                        owl:allValuesFrom [ owl:unionOf ( foaf:Person foaf:Organization ) ]
                                      ] ,
                                      [ rdf:type owl:Restriction ;
                                        owl:onProperty schema:author ;
                                        owl:allValuesFrom [ owl:unionOf ( foaf:Person foaf:Organization ) ]
                                      ] ,
                                      [ rdf:type owl:Restriction ;
                                        owl:onProperty schema:inLanguage ;
                                        owl:someValuesFrom schema:Language
                                      ] ,
                                      [ rdf:type owl:Restriction ;
                                        owl:onProperty schema:datePublished ;
                                        owl:maxCardinality "1"^^xsd:nonNegativeInteger
                                      ] ,
                                      [ rdf:type owl:Restriction ;
                                        owl:onProperty schema:dateModified ;
                                        owl:maxCardinality "1"^^xsd:nonNegativeInteger
                                      ] ,
                                      [ rdf:type owl:Restriction ;
                                        owl:onProperty schema:version ;
                                        owl:maxCardinality "1"^^xsd:nonNegativeInteger
                                      ] ,
                                      [ rdf:type owl:Restriction ;
                                        owl:onProperty schema:publisher ;
                                        owl:allValuesFrom [ owl:unionOf ( foaf:Person foaf:Organization ) ]
                                      ] ,
                                      [ rdf:type owl:Restriction ;
                                        owl:onProperty triple:aggregator ;
                                        owl:allValuesFrom [ owl:unionOf ( foaf:Person foaf:Organization ) ]
                                      ] ,
                                      [ rdf:type owl:Restriction ;
                                        owl:onProperty schema:fileFormat ;
                                        owl:someValuesFrom xsd:string
                                      ] ,
                                      [ rdf:type owl:Restriction ;
                                        owl:onProperty schema:encodingFormat ;
                                        owl:someValuesFrom xsd:string
                                      ] ,
                                      [ rdf:type owl:Restriction ;
                                        owl:onProperty schema:contactPoint ;
                                        owl:allValuesFrom schema:ContactPoint
                                      ] ,
                                      [ rdf:type owl:Restriction ;
                                        owl:onProperty schema:creativeWorkStatus ;
                                        owl:maxCardinality "1"^^xsd:nonNegativeInteger
                                      ] ,
                                      [ rdf:type owl:Restriction ;
                                        owl:onProperty schema:keywords ;
                                        owl:allValuesFrom schema:DefinedTerm
                                      ] ,
                                      [ rdf:type owl:Restriction ;
                                        owl:onProperty dcterms:isReferencedBy ;
                                        owl:allValuesFrom triple:Document
                                      ] ,
                                      [ rdf:type owl:Restriction ;
                                        owl:onProperty datacite:hasIdentifier ;
                                        owl:allValuesFrom datacite:Identifier
                                      ] ,
                                      [ rdf:type owl:Restriction ;
                                        owl:onProperty schema:spatialCoverage ;
                                        owl:allValuesFrom schema:Place
                                      ] .


#################################################################
#    Individuals
#################################################################

###  https://gotriple.eu/ontology/triple#doi
triple:doi rdf:type owl:NamedIndividual ,
                   datacite:IdentifierScheme ;
          rdfs:label "DOI" ;
          rdfs:comment "Digital Object Identifier - a persistent identifier for digital objects maintained by the International DOI Foundation"@en .

###  https://gotriple.eu/ontology/triple#handle
triple:handle rdf:type owl:NamedIndividual ,
                      datacite:IdentifierScheme ;
             rdfs:label "Handle" ;
             rdfs:comment "Handle System - a persistent identifier infrastructure for managing digital objects"@en .

###  https://gotriple.eu/ontology/triple#uri
triple:uri rdf:type owl:NamedIndividual ,
                   datacite:IdentifierScheme ;
          rdfs:label "URI" ;
          rdfs:comment "Uniform Resource Identifier - a string of characters that unambiguously identifies a particular resource"@en .

###  https://gotriple.eu/ontology/triple#landing_page_url
triple:landing_page_url rdf:type owl:NamedIndividual ,
                                 datacite:IdentifierScheme ;
                        rdfs:label "Landing Page URL"@en ;
                        rdfs:comment "URL of the landing page containing metadata and descriptive information about the document."@en .


###  https://gotriple.eu/ontology/triple#full_text_url
triple:full_text_url rdf:type owl:NamedIndividual ,
                              datacite:IdentifierScheme ;
                     rdfs:label "Full Text URL"@en ;
                     rdfs:comment "URL providing direct access to the full content of the document."@en .


###  https://gotriple.eu/ontology/triple#source_url
triple:source_url rdf:type owl:NamedIndividual ,
                           datacite:IdentifierScheme ;
                  rdfs:label "Source URL"@en ;
                  rdfs:comment "URL of the original publication location or source repository."@en .


###  https://gotriple.eu/ontology/triple#internal_id
triple:internal_id rdf:type owl:NamedIndividual ,
                            datacite:IdentifierScheme ;
                   rdfs:label "Internal ID"@en ;
                   rdfs:comment "Internal identifier used within the GoTriple platform for document management."@en .


###  https://gotriple.eu/ontology/triple#pid
triple:pid rdf:type owl:NamedIndividual ,
                    datacite:IdentifierScheme ;
           rdfs:label "PID"@en ;
           rdfs:comment "Persistent identifier generated and exposed externally by the GoTriple platform."@en .


###  https://gotriple.eu/ontology/triple#original_id
triple:original_id rdf:type owl:NamedIndividual ,
                            datacite:IdentifierScheme ;
                   rdfs:label "Original ID"@en ;
                   rdfs:comment "Original identifier from the source system where the document was harvested."@en .
